Projects/AP/Reachability.lean
@@ -2,39 +2,39 @@ import Projects.AP.WF
 
 namespace AP
 
-def State.diff (s₁ s : State) : ℕ :=
+def State.diff (s s₁ : State) : ℕ :=
   s₁.hist.length - s.hist.length
 
-def State.diffTrs (s₁ s : State) : List PointZ :=
-  s₁.hist.take (s₁.diff s) |>.reverse
+def State.diffTrs (s s₁ : State) : List PointZ :=
+  s₁.hist.take (s.diff s₁) |>.reverse
 
 def State.isReachable (s₁ s₂ : State) : Bool :=
-  sys.trs s₁ (s₂.diffTrs s₁) == (s₂, [])
+  sys.trs s₁ (s₁.diffTrs s₂) == (s₂, [])
 
-def State.exiSimulate (s : State) (f : State → PointZ) (s₁ : State) : Bool :=
-  sys.simulate f s (s₁.diff s) = (s₁, 0)
+def State.exiSimulate (f : State → PointZ) (s : State) (s₁ : State) : Bool :=
+  sys.simulate f s (s.diff s₁) = (s₁, 0)
 
 -- #check 0 #exit
 
 -----
 
 theorem State.diff_eq_of_simulate' {s f n s₁ r}
-(h : sys.simulate f s n = (s₁, r)) : s₁.diff s + r = n := by
+(h : sys.simulate f s n = (s₁, r)) : s.diff s₁ + r = n := by
   unfold diff
   rw [length_hist_eq_of_simulate_eq h]
   have h₁ := sys.snd_le_of_simulate_eq h
   omega
 
 theorem State.diff_eq_of_simulate {s f n s₁ r}
-(h : sys.simulate f s n = (s₁, r)) : s₁.diff s = n - r := by
+(h : sys.simulate f s n = (s₁, r)) : s.diff s₁ = n - r := by
   have := diff_eq_of_simulate' h; omega
 
 theorem State.diff_eq_of_simulate_full {s f n s₁}
-(h : sys.simulate f s n = (s₁, 0)) : s₁.diff s = n :=
+(h : sys.simulate f s n = (s₁, 0)) : s.diff s₁ = n :=
   diff_eq_of_simulate h
 
 @[simp]
-theorem State.length_diffTrs {s s₁ : State} : (s₁.diffTrs s).length = s₁.diff s := by
+theorem State.length_diffTrs {s s₁ : State} : (s.diffTrs s₁).length = s.diff s₁ := by
   simp [diffTrs, diff]
 
 @[simp]
@@ -46,15 +46,15 @@ theorem State.diffTrs_self {s : State} : s.diffTrs s = [] := by
   simp [diffTrs]
 
 theorem State.diff_eq_of_tr {s s₁ s₂ p} (h : sys.tr s₁ p = some s₂)
-(h₁ : sys.Reachable s s₁) : s₂.diff s = s₁.diff s + 1 := by
+(h₁ : sys.Reachable s s₁) : s.diff s₂ = s.diff s₁ + 1 := by
   simp [diff, length_hist_eq_of_tr h]; have := length_hist_le_of_reachable h₁; omega
 
 theorem State.diffTrs_eq_of_tr {s s₁ s₂ p} (h : sys.tr s₁ p = some s₂)
-(h₁ : sys.Reachable s s₁) : s₂.diffTrs s = s₁.diffTrs s ++ [p] := by
+(h₁ : sys.Reachable s s₁) : s.diffTrs s₂ = s.diffTrs s₁ ++ [p] := by
   simp [diffTrs, diff_eq_of_tr h h₁, hist_eq_of_tr h]
 
 theorem State.diffTrs_eq_of_trs_full {s ps s₁}
-(h : sys.trs s ps = (s₁, [])) : s₁.diffTrs s = ps := by
+(h : sys.trs s ps = (s₁, [])) : s.diffTrs s₁ = ps := by
   induction ps using List.reverseRecOn generalizing s₁
   · simp at h; simp [h]
   nm ps p ih
@@ -109,7 +109,7 @@ s.exiSimulate f s₁ = decide (∃ n, sys.simulate f s n = (s₁, 0)) := by
   simp [exi_simulate_iff_exiSimulate]
 
 theorem State.diff_eq_of_trs_full {s ps s₁}
-(h : sys.trs s ps = (s₁, [])) : s₁.diff s = ps.length := by
+(h : sys.trs s ps = (s₁, [])) : s.diff s₁ = ps.length := by
   rw [←length_diffTrs, diffTrs_eq_of_trs_full h]
 
 @[simp]
