Projects/AP/Moves/Defs.lean
@@ -1,0 +1,138 @@
+import Projects.AP.Reachability
+
+namespace AP
+
+-- Given function `f` and states `s` and `s₁`,
+-- determines whether `s₁` is reachable from `s` via `f`
+def State.ReachableVia' (f : State → PointZ) (s s₁ : State) : Prop :=
+  ∃ n, sys.simulate f s n = (s₁, 0)
+
+-- Given strategy `st` and states `s` and `s₁`,
+-- determines whether `s₁` is reachable from `s` via `st`
+def State.ReachableVia (st : Strat) (s s₁ : State) : Prop :=
+  s.ReachableVia' st.f s₁
+
+instance {s s₁ : State} {st} : Decidable # s.ReachableVia st s₁ := by
+  apply decidable_of_bool # sys.simulate st.f s (s.diff s₁) = (s₁, 0)
+  simp [State.ReachableVia, State.ReachableVia']; constructor; tauto
+  rintro ⟨n, h⟩; simpa [State.diff_eq_of_simulate h]
+
+-- Given start state `s`, strategy `st` and future state `s₁`,
+-- if `s₁` can be reached from `s` via `st`,
+-- returns either A move or D move performed is `s₁`
+def State.moveSim (s : State) (st : Strat) (s₁ : State) :
+Option # (PointZ × State) ⊕ (PointZ × State) := do
+  guard # s.ReachableVia st s₁
+  let p := st.f s₁
+  let s₂ ← sys.tr s₁ p
+  pure # ite s₁.aTurn Sum.inr Sum.inl (p, s₂)
+
+-- Given start state `s`, strategy `st` and future state `s₁`,
+-- if `s₁` is A state and can be reached from `s` via `st`,
+-- returns A move performed in `s₁`
+def State.aMoveSim (s : State) (st : Strat) (s₁ : State) : Option (PointZ × State) := do
+  match ← s.moveSim st s₁ with
+  | .inr r => some r
+  | _ => none
+
+-- Given start state `s`, strategy `st` and future state `s₁`,
+-- if `s₁` is D state and can be reached from `s` via `st`,
+-- returns D move performed in `s₁`
+def State.dMoveSim (s : State) (st : Strat) (s₁ : State) : Option (PointZ × State) := do
+  match ← s.moveSim st s₁ with
+  | .inl r => some r
+  | _ => none
+
+-- Given state `s` and strategy `st`,
+-- returns the set of all future A states and moves at these states
+def State.aSimPairs (s : State) (st : Strat) : Set (State × PointZ) :=
+  {(s₁, p) | ∃ s₂, s.aMoveSim st s₁ = some (p, s₂)}
+
+-- Given state `s` and strategy `st`,
+-- returns the set of all future A moves
+def State.aSimPts (s : State) (st : Strat) : Set PointZ :=
+  Prod.snd '' s.aSimPairs st
+
+-- Given state `s` and strategy `st`,
+-- returns the set of all future states
+def State.simStates (s : State) (st : Strat) : Set State :=
+  setOf # s.ReachableVia st
+
+def State.simStatesRangeAuxVia (r : ℕ → ℕ → Prop) [hs : DecidableRel r]
+(st : Strat) (s s₁ : State) : Finset State :=
+  if ¬s.ReachableVia st s₁ then ∅ else
+  Finset.Icc 0 (s.diff s₁) |>.image (λ n => sys.simulate st.f s n |>.1)
+    |>.filter λ s₂ => r s₂.hist.length s₁.hist.length
+
+-- Interval of states `[s, s₁]` via strategy `st`
+def State.simStatesIccVia (st : Strat) (s s₁ : State) : Finset State :=
+  s.simStatesRangeAuxVia (· ≤ ·) st s₁
+
+-- Interval of states `[s, s₁)` via strategy `st`
+def State.simStatesIcoVia (st : Strat) (s s₁ : State) : Finset State :=
+  s.simStatesRangeAuxVia (· < ·) st s₁
+
+-- A states in interval `[s, s₁]` via strategy `st`
+def State.aSimStatesIccVia (st : Strat) (s s₁ : State) : Finset State :=
+  s.simStatesIccVia st s₁ |>.filter (·.aTurn)
+
+-- A states in interval `[s, s₁)` via strategy `st`
+def State.aSimStatesIcoVia (st : Strat) (s s₁ : State) : Finset State :=
+  s.simStatesIcoVia st s₁ |>.filter (·.aTurn)
+
+-- Set of all future A states via strategy `st`
+def State.aSimStates (s : State) (st : Strat) : Set State :=
+  s.simStates st |>.filter (·.aTurn)
+
+-- Initial state of the given state
+def State.init (s : State) : State :=
+  initState s.pw s.aPos₀
+
+-- Previous state
+def State.prev (s : State) : State :=
+  sys.trs s.init (s.init.diffTrs s |>.init) |>.1
+
+-- Last move
+def State.lastMove (s : State) : PointZ :=
+  s.prev.diffTrs s |>.getLast!
+
+-- Checks whether the state is initial
+def State.IsInit (s : State) : Prop :=
+  sys.Initial s
+
+-- The cardinality of the set of all future A moves
+noncomputable
+def State.aSimPtsNcard (s : State) (st : Strat) (set : Set PointZ) : Option ℕ :=
+  s.aSimPairs st |>.filter (·.2 ∈ set) |>.ncard?
+
+-- Create a strategy from a function
+def Strat.ofFn (f : State → Option PointZ) : Strat where
+  a := .mk f
+  d := .mk f
+
+-- Returns a strategy that goes from `s` to `s₁` (if it exists)
+def State.diffStrat (s s₁ : State) : Strat :=
+  .ofFn λ s' => (s.diffTrs s₁)[s.diff s']?
+
+-- #check 0 #exit
+
+def State.aVisitedIcc' (s : State) (ps : List PointZ) : Set' PointZ :=
+  match ps with
+  | [] => ∅
+  | p :: ps =>
+    let set := sys.tr s p |>.getd.aVisitedIcc' ps
+    if s.aTurn then set.insert p else set
+
+-- Set of all `aPos` from `[s, s₁]`
+def State.aVisitedIcc (s s₁ : State) : Set' PointZ :=
+  if sys.Reachable s s₁ then State.aVisitedIcc' s (s.diffTrs s₁) |>.insert s.aPos else ∅
+
+-- Set of all `aPos` from `[s, s₁)`
+def State.aVisitedIco (s s₁ : State) : Set' PointZ :=
+  if s = s₁ then ∅ else s.aVisitedIcc s₁.prev
+
+def State.aVisitedIcoPrev (s s₁ : State) : Set' PointZ :=
+  if s.diff s₁ ≤ 1 then ∅ else s.aVisitedIco s₁.prev
+
+def State.aNbhdsIcoPrev (s s₁ : State) : Set' PointZ :=
+  s.aVisitedIcoPrev s₁ |>.bind (·.nbhd s.pw)
