Projects/AP/Moves/Part_001.lean
@@ -1,0 +1,1395 @@
+import Projects.AP.Moves.Defs
+
+namespace AP
+
+@[simp]
+theorem State.aVisitedIcc'_nil {s : State} : s.aVisitedIcc' [] = ∅ := rfl
+
+@[simp]
+theorem State.aVisitedIcc_self {s : State} : s.aVisitedIcc s = Set'.singleton s.aPos := by
+  simp [aVisitedIcc]
+
+theorem State.aTurn_iff_aState {s} [hs : sys.WF s] : s.aTurn ↔ AState s := by
+  constructor
+  · intro h; use hs
+  · intro h; simp
+
+@[simp]
+theorem State.aVisitedIcc'_singleton {s : State} {p} :
+s.aVisitedIcc' [p] = if s.aTurn then Set'.singleton p else ∅ := by
+  simp [aVisitedIcc']
+
+theorem AState.aVisitedIcc'_cons {s s' : State} {p ps} [hs : AState s]
+(h : sys.tr s p = some s') : s.aVisitedIcc' (p :: ps) =
+(s'.aVisitedIcc' ps).insert p := by
+  simp [State.aVisitedIcc', h]
+
+theorem DState.aVisitedIcc'_cons {s s' : State} {p ps} [hs : DState s]
+(h : sys.tr s p = some s') : s.aVisitedIcc' (p :: ps) = s'.aVisitedIcc' ps := by
+  simp [State.aVisitedIcc', h]
+
+theorem AState.aVisitedIcc'_snoc {s s₁ : State} {ps p} [hs : sys.WF s]
+[hs₁ : AState s₁] (h₁ : sys.trs s ps = (s₁, [])) :
+s.aVisitedIcc' (ps ++ [p]) = (s.aVisitedIcc' ps).insert p := by
+  induction ps generalizing s
+  · simp at h₁; simp [h₁]
+  nm p₁ ps ih
+  simp at h₁
+  choose s' h₁ h₃ using h₁
+  have hs' := sys.wf_of_tr h₁
+  specialize ih h₃
+  replace hs := s.aState_or_dState
+  rw [List.cons_append]
+  rcases hs with hs | hs
+  · simp_rw [AState.aVisitedIcc'_cons h₁, ih, Set'.insert_comm]
+  · simp_rw [DState.aVisitedIcc'_cons h₁, ih]
+
+theorem DState.aVisitedIcc'_snoc {s s₁ : State} {ps p} [hs : sys.WF s]
+[hs₁ : DState s₁] (h₁ : sys.trs s ps = (s₁, [])) :
+s.aVisitedIcc' (ps ++ [p]) = s.aVisitedIcc' ps := by
+  induction ps generalizing s
+  · simp at h₁; simp [h₁]
+  nm p₁ ps ih
+  simp at h₁
+  choose s' h₁ h₃ using h₁
+  have hs' := sys.wf_of_tr h₁
+  specialize ih h₃
+  replace hs := s.aState_or_dState
+  rw [List.cons_append]
+  rcases hs with hs | hs
+  · simp_rw [AState.aVisitedIcc'_cons h₁, ih]
+  · simp_rw [DState.aVisitedIcc'_cons h₁, ih]
+
+theorem AState.aVisitedIcc_eq_of_tr {s s₁ s₂ p} [hs : sys.WF s] [hs₁ : AState s₁]
+(h : sys.tr s₁ p = some s₂) (h₁ : sys.Reachable s s₁) :
+s.aVisitedIcc s₂ = (s.aVisitedIcc s₁).insert p := by
+  rw [sys.reachable_iff_exi_trs] at h₁
+  choose ps h₁ using h₁
+  simp [State.aVisitedIcc]
+  rw [State.diffTrs_eq_of_trs_full h₁]
+  have h₂ : sys.trs s (ps ++ [p]) = (s₂, [])
+  · simpa [h₁]
+  rw [if_pos # sys.reachable_of_trs h₁]
+  rw [if_pos # sys.reachable_of_trs h₂]
+  rw [State.diffTrs_eq_of_trs_full h₂, Set'.insert_comm]
+  rw [aVisitedIcc'_snoc h₁]
+
+theorem DState.aVisitedIcc_eq_of_tr {s s₁ s₂ p} [hs : sys.WF s] [hs₁ : DState s₁]
+(h : sys.tr s₁ p = some s₂) (h₁ : sys.Reachable s s₁) :
+s.aVisitedIcc s₂ = s.aVisitedIcc s₁ := by
+  rw [sys.reachable_iff_exi_trs] at h₁
+  choose ps h₁ using h₁
+  simp [State.aVisitedIcc]
+  rw [State.diffTrs_eq_of_trs_full h₁]
+  have h₂ : sys.trs s (ps ++ [p]) = (s₂, [])
+  · simpa [h₁]
+  rw [if_pos # sys.reachable_of_trs h₁]
+  rw [if_pos # sys.reachable_of_trs h₂]
+  rw [State.diffTrs_eq_of_trs_full h₂]
+  rw [aVisitedIcc'_snoc h₁]
+
+theorem State.mem_aVisitedIcc_iff_of {s f n s₁ p} [hs : sys.WF s]
+(h : sys.simulate f s n = (s₁, 0)) : p ∈ s.aVisitedIcc s₁ ↔ p = s.aPos ∨
+∃ k < n, ∃ s', AState s' ∧ sys.simulate f s k = (s', 0) ∧ f s' = p := by
+  induction n generalizing s₁
+  · simp at h; simp [h]
+  nm n ih
+  simp at h
+  choose s' h₁ h₂ using h
+  specialize ih h₁
+  have hs' : sys.WF s'; grind
+  have hs₁ : sys.WF s₁; grind
+  have h₃ := sys.reachable_of_simulate h₁
+  replace hs' := s'.aState_or_dState
+  rcases hs' with hs' | hs'
+  all_goals simp [hs'.aVisitedIcc_eq_of_tr h₂ h₃, ih]; clear ih
+  · grind
+  apply iff_of_eq; congr 1; apply propext
+  apply exists_congr; intro k
+  by_cases h : k ≠ n
+  · simp [le_iff_eq_or_lt, h]
+  push_neg at h; subst h
+  simp
+  rintro s₂ hs₂ h₄ rfl
+  simp [h₁] at h₄
+  contrapose! h₄
+  apply ne_of_congr (·.aTurn); simp
+
+theorem State.trs_diffTrs {s s₁ ps ps'} [hs : sys.WF s]
+(h : sys.trs s ps = (s₁, ps')) : sys.trs s (s.diffTrs s₁) = (s₁, []) := by
+  induction ps using List.reverseRecOn generalizing s s₁ ps'
+  · simp at h; simp [h]
+  nm ps p ih
+  simp [sys.trs_append] at h
+  generalize hr : sys.trs s ps = r at h
+  rcases r with ⟨s', r⟩
+  dsimp at h
+  split_ifs at h with h₁
+  · subst h₁
+    simp at h
+    specialize ih hr
+    simp [System.trs] at h
+    split at h
+    · grind
+    nm x s₂ h₁; clear x
+    simp at h
+    rcases h with ⟨rfl, rfl⟩
+    rw [diffTrs_eq_of_tr h₁ # sys.reachable_of_trs hr]
+    simpa [ih]
+  simp at h
+  rcases h with ⟨rfl, rfl⟩
+  exact ih hr
+
+theorem State.simulate_diff {s s₁ f n r} [hs : sys.WF s]
+(h : sys.simulate f s n = (s₁, r)) : sys.simulate f s (s.diff s₁) = (s₁, 0) := by
+  induction n generalizing s s₁ r
+  · simp at h; simp [h]
+  nm n ih
+  rw [sys.simulate_add] at h
+  simp at h
+  generalize hr : sys.simulate f s n = r at h
+  rcases r with ⟨s', r⟩
+  dsimp at h
+  split_ifs at h with h₁
+  · subst h₁
+    simp at h
+    specialize ih hr
+    simp [System.simulate] at h
+    split at h
+    · grind
+    nm x s₂ h₁; clear x
+    simp at h
+    rcases h with ⟨rfl, rfl⟩
+    rw [diff_eq_of_tr h₁ # by grind]
+    rw [sys.simulate_add]
+    simpa [ih]
+  simp at h
+  rcases h with ⟨rfl, rfl⟩
+  exact ih hr
+
+theorem State.aSimPts_eq_setOf {s : State} {st} : s.aSimPts st =
+{p | ∃ s₁ s₂, s.aMoveSim st s₁ = some (p, s₂)} := by
+  ext; simp [aSimPts, aSimPairs]
+
+theorem State.mem_aSimPts_iff_aSimPairs {s : State} {st p} :
+p ∈ s.aSimPts st ↔ ∃ s₁, (s₁, p) ∈ s.aSimPairs st := by
+  simp [aSimPts]
+
+@[simp]
+theorem State.mem_simStates_iff {s : State} {st s₁} :
+s₁ ∈ s.simStates st ↔ s.ReachableVia st s₁ := by rfl
+
+theorem State.false_of_aState_and_dState s [hs₁ : AState s] [hs₂ : DState s] : False := by
+  simp at hs₁
+
+theorem AState.even_of_simulate {s s₁ f n} [hs : AState s] [hs₁ : AState s₁]
+(h : sys.simulate f s n = (s₁, 0)) : Even n := by
+  by_contra h₁; simp at h₁
+  obtain ⟨n, rfl⟩ := h₁
+  rw [mul_comm] at h
+  have h₁ := DState.of_simulate_mul_two_add_one_eq_full h
+  exact s₁.false_of_aState_and_dState
+
+theorem AState.odd_of_simulate {s s₁ f n} [hs : AState s] [hs₁ : DState s₁]
+(h : sys.simulate f s n = (s₁, 0)) : Odd n := by
+  by_contra h₁; simp at h₁; obtain ⟨n, rfl⟩ := Nat.even_iff_exi.mp h₁
+  have h₂ := AState.of_simulate_mul_two_eq_full h; simp at h₂
+
+theorem DState.even_of_simulate {s s₁ f n} [hs : DState s] [hs₁ : DState s₁]
+(h : sys.simulate f s n = (s₁, 0)) : Even n := by
+  by_contra h₁; simp at h₁
+  obtain ⟨n, rfl⟩ := Nat.odd_iff_exi.mp h₁; clear h₁
+  simp at h
+  choose s' h₁ h₂ using h
+  have : sys.WF s'; grind
+  have : AState s'; grind
+  have h₃ := DState.of_simulate_mul_two_eq_full h₁
+  simp at h₃
+
+theorem DState.odd_of_simulate {s s₁ f n} [hs : DState s] [hs₁ : AState s₁]
+(h : sys.simulate f s n = (s₁, 0)) : Odd n := by
+  by_contra h₁; simp at h₁
+  obtain ⟨n, rfl⟩ := Nat.even_iff_exi.mp h₁; clear h₁
+  have h₁ := DState.of_simulate_mul_two_eq_full h
+  simp at h₁
+
+@[simp]
+theorem State.mem_aSimStates_iff {s : State} {st s₁} [hs : sys.WF s] :
+s₁ ∈ s.aSimStates st ↔ AState s₁ ∧ ∃ n, sys.simulate st.f s n = (s₁, 0) := by
+  simp [aSimStates]
+  constructor
+  · rintro ⟨⟨n, h⟩, hs₁'⟩
+    have hs₁ : sys.WF s₁; grind
+    replace hs₁ : AState s₁; grind
+    use hs₁, n
+  · rintro ⟨hs₁1, n, h⟩; simp; use n
+
+theorem State.mem_aSimPairs_iff_simulate_tr {s s₁ p} {st : Strat} [hs : sys.WF s] :
+(s₁, p) ∈ s.aSimPairs st ↔ AState s₁ ∧ ∃ n, sys.simulate st.f s n = (s₁, 0) ∧
+∃ s₂, sys.tr s₁ (st.a.f s₁) = some s₂ ∧ st.a.f s₁ = p := by
+  simp only [aSimPairs, aMoveSim, moveSim, Option.pure_def, Option.bind_eq_bind,
+    Option.bind_eq_some_iff', Option.guard_eq_some', Option.some.injEq, exists_const, Sum.exists,
+    reduceCtorEq, and_false, exists_eq_right, false_or, exists_and_left, Set.mem_setOf_eq,
+    exists_and_right]
+  unfold ReachableVia ReachableVia'; constructor
+  · rintro ⟨h₁, s₂, s₃, h₂, h₃⟩
+    split_ifs at h₃ with ht
+    simp at h₃
+    rcases h₃ with ⟨rfl, rfl⟩
+    apply and_of
+    · constructor <;> grind
+    intro hs₁
+    clear ht
+    simp
+    generalize hr : sys.simulate st.f s (s.diff s₁) = r at h₁ ⊢
+    rcases r with ⟨s₁, r⟩
+    rcases h₁ with ⟨n, h₁⟩
+    simp [h₁, diff_eq_of_simulate h₁] at hr
+    rcases hr with ⟨rfl, rfl⟩
+    simp at h₂ ⊢; simp [h₂]; use n
+  · rintro ⟨hs₁, ⟨n, h₁⟩, ⟨s₂, h₂⟩, rfl⟩
+    simp; tauto
+
+theorem State.mem_aSimPts_iff_simulate_tr {s p} {st : Strat} [hs : sys.WF s] :
+p ∈ s.aSimPts st ↔ ∃ n s₁, AState s₁ ∧ sys.simulate st.f s n = (s₁, 0) ∧
+∃ s₂, sys.tr s₁ (st.a.f s₁) = some s₂ ∧ st.a.f s₁ = p := by
+  simp_rw [mem_aSimPts_iff_aSimPairs, mem_aSimPairs_iff_simulate_tr]; grind
+
+theorem State.mem_aSimPts_iff_simulate_ge_two {s p} {st : Strat} [hst : st.WF] [hs : sys.WF s] :
+p ∈ s.aSimPts st ↔ ∃ n s₁, 2 ≤ n ∧ sys.simulate st.f s n = (s₁, 0) ∧ s₁.aPos = p := by
+  rw [mem_aSimPts_iff_simulate_tr]
+  constructor
+  · rintro ⟨n, s₁, hs₁, h₁, s₂, h₂, rfl⟩
+    have hs₂ := DState.of_tr h₂
+    obtain ⟨s₃, h₃⟩ : sys.validTr s₂ (st.d.f s₂)
+    · simp
+    use n + 2, by omega
+    rw [sys.simulate_add]
+    simp [System.simulate, h₁, h₂, h₃]
+    rw [DState.aPos_eq_of_tr h₃, AState.aPos_eq_of_tr h₂]
+  · rintro ⟨n, s₃, hn, h₁, rfl⟩
+    simp only [exists_and_right]
+    obtain ⟨n, rfl⟩ := Nat.exists_eq_add_of_le hn; clear hn
+    rw [add_comm] at h₁
+    simp at h₁
+    obtain ⟨s₂, ⟨s₁, h₁, h₂⟩, h₃⟩ := h₁
+    have hs₁ : sys.WF s₁; grind
+    replace hs₁ := s₁.aState_or_dState
+    rcases hs₁ with hs₁ | hs₁
+    · simp at h₂
+      have hs₂ := DState.of_tr h₂
+      use n, s₁, hs₁, h₁
+      refine ⟨⟨s₂, h₂⟩, ?_⟩
+      rw [DState.aPos_eq_of_tr h₃, AState.aPos_eq_of_tr h₂]
+    · have hs₂ := AState.of_tr h₂
+      simp at h₂ h₃
+      use n + 1, s₂, hs₂
+      rw [sys.simulate_add]
+      simp [h₁]
+      use h₂
+      refine ⟨⟨s₃, h₃⟩, ?_⟩
+      rw [AState.aPos_eq_of_tr h₃]
+
+theorem State.aVisitedIcc_subset_of_simulate_le  (st : Strat) k n {s s₁ s₂} [hs : sys.WF s]
+(hn : k ≤ n) (h₁ : sys.simulate st.f s k = (s₁, 0)) (h₂ : sys.simulate st.f s n = (s₂, 0)) :
+s.aVisitedIcc s₁ ⊆ s.aVisitedIcc s₂ := by
+  intro p; rw [mem_aVisitedIcc_iff_of h₁, mem_aVisitedIcc_iff_of h₂]; grind
+
+@[simp, grind ·]
+instance {s : State} : sys.Initial s.init := by
+  unfold State.init; infer_instance
+
+@[simp]
+theorem State.one_le_hist_length {s} [hs : sys.WF s] : 1 ≤ s.hist.length := by
+  simp [Nat.one_le_iff_ne_zero]
+
+theorem State.diff_init_succ {s} [hs : sys.WF s] : s.init.diff s + 1 = s.hist.length := by
+  simp [init, diff]
+
+@[simp]
+theorem State.diff_init {s} [hs : sys.WF s] : s.init.diff s = s.hist.length - 1 := by
+  have := s.diff_init_succ; omega
+
+@[simp]
+theorem State.isInit_initial {s} [hs : sys.Initial s] : s.IsInit := hs
+
+theorem State.isInit_of_length_hist_eq_one {s}
+[hs : sys.WF s] (h : s.hist.length = 1) : s.IsInit := by
+  rw [IsInit, initial_iff]; ext <;> simp_all
+
+theorem State.length_hist_eq_one_of_isInit {s : State}
+(h : s.IsInit) : s.hist.length = 1 := by
+  rw [IsInit, initial_iff] at h; rw [←h]; rfl
+
+theorem State.isInit_iff_length_hist_eq_one {s}
+[hs : sys.WF s] : s.IsInit ↔ s.hist.length = 1 :=
+  ⟨length_hist_eq_one_of_isInit, isInit_of_length_hist_eq_one⟩
+
+@[simp]
+theorem State.length_hist_init {s : State} : s.init.hist.length = 1 := by
+  simp [init]
+
+@[simp]
+theorem State.diffTrs_init {s} [hs : sys.WF s] : s.init.diffTrs s = s.hist.init.reverse := by
+  simp [diffTrs]
+
+@[simp]
+theorem AState.initState_ne {s pw p₀} [ha : AState s] : initState pw p₀ ≠ s := by
+  rintro rfl; simp at ha
+
+@[simp]
+theorem AState.not_isInit {s} [ha : AState s] : ¬s.IsInit := by
+  simp [State.IsInit]
+
+theorem State.wf_prev_and_tr {s} [hs : sys.WF s]
+(h : ¬s.IsInit) : sys.WF s.prev ∧ sys.tr s.prev s.lastMove = some s := by
+  choose ps h₁ using wf_iff'.mp hs
+  induction ps using List.reverseRecOn
+  · simp at h₁
+    rw [←h₁] at h
+    simp at h
+  nm ps p ih; clear ih
+  simp at h₁
+  choose s' h₁ h₂ using h₁
+  rw [lastMove, prev]
+  simp [hist_eq_of_tr h₂, hist_eq_of_trs h₁]
+  simp [init, h₁, diffTrs_eq_of_tr h₂, h₂]
+  exact sys.wf_of_trs h₁
+
+theorem State.wf_prev {s} [hs : sys.WF s] (h : ¬s.IsInit) : sys.WF s.prev :=
+  wf_prev_and_tr h |>.1
+
+theorem State.prev_tr_lastMove {s} [hs : sys.WF s]
+(h : ¬s.IsInit) : sys.tr s.prev s.lastMove = some s :=
+  wf_prev_and_tr h |>.2
+
+theorem State.length_hist_prev {s} [hs : sys.WF s]
+(h : ¬s.IsInit) : s.prev.hist.length = s.hist.length - 1 := by
+  simp [length_hist_eq_of_tr # prev_tr_lastMove h]
+
+theorem State.not_isInit_of_tr {s s' p} [hs : sys.WF s]
+(h : sys.tr s p = some s') : ¬s'.IsInit := by
+  have hs' := sys.wf_of_tr h; simp [isInit_iff_length_hist_eq_one, length_hist_eq_of_tr h]
+
+theorem State.eq_iff_pw_and_hist {s₁ s₂} [hs₁ : sys.WF s₁] [hs₂ : sys.WF s₂] :
+s₁ = s₂ ↔ s₁.pw = s₂.pw ∧ s₁.hist = s₂.hist := by
+  use by rintro rfl; simp;
+  rintro ⟨h₁, h₂⟩
+  choose ps₁ h₃ using wf_iff'.mp hs₁
+  choose ps₂ h₄ using wf_iff'.mp hs₂
+  rw [←h₁, aPos₀, ←h₂, ←aPos₀] at h₄
+  simp [hist_eq_of_trs h₃, hist_eq_of_trs h₄] at h₂
+  grind
+
+theorem State.tr_inj {s₁ s₂ s₃ p₁ p₂} [hs₁ : sys.WF s₁] [hs₂ : sys.WF s₂]
+(h₁ : sys.tr s₁ p₁ = some s₃) (h₂ : sys.tr s₂ p₂ = some s₃) : s₁ = s₂ ∧ p₁ = p₂ := by
+  replace hs₁ := s₁.aState_or_dState
+  rcases hs₁ with hs₁ | hs₁
+  · have hs₃ := DState.of_tr h₁
+    replace hs₂ := AState.of_tr' h₂
+    rw [AState.tr_eq_some_iff] at h₁ h₂
+    rcases h₂ with ⟨⟨h₄, h₅, h₆⟩, rfl⟩
+    rcases h₁ with ⟨⟨h₁, h₂, h₃⟩, h₇⟩
+    rw [eq_iff_pw_and_hist]; grind
+  · have hs₃ := AState.of_tr h₁
+    replace hs₂ := DState.of_tr' h₂
+    rw [DState.tr_eq_some_iff] at h₁ h₂
+    rcases h₂ with ⟨⟨h₄, h₅⟩, rfl⟩
+    rcases h₁ with ⟨⟨h₁, h₂⟩, h₇⟩
+    rw [eq_iff_pw_and_hist]; grind
+
+theorem State.lastMove_eq_of_tr {s s' p} [hs : sys.WF s]
+(h : sys.tr s p = some s') : s'.lastMove = p := by
+  have hs' := sys.wf_of_tr h
+  have h₁ := not_isInit_of_tr h
+  have h₂ := prev_tr_lastMove h₁
+  have H := wf_prev h₁
+  obtain ⟨rfl, rfl⟩ := tr_inj h h₂; rfl
+
+theorem State.diffTrs_prev {s} [hs : sys.WF s]
+(h : ¬s.IsInit) : s.prev.diffTrs s = [s.lastMove] := by
+  simp [diffTrs_eq_of_tr # prev_tr_lastMove h]
+
+theorem State.diff_prev {s} [hs : sys.WF s]
+(h : ¬s.IsInit) : s.prev.diff s = 1 := by
+  simp [diff_eq_of_tr # prev_tr_lastMove h]
+
+theorem State.prev_eq_of_tr {s s' p} [hs : sys.WF s]
+(h : sys.tr s p = some s') : s'.prev = s := by
+  have hs' := sys.wf_of_tr h
+  have H₁ := not_isInit_of_tr h
+  have h₁ := s'.prev_tr_lastMove H₁
+  have H₂ := wf_prev H₁
+  obtain ⟨rfl, rfl⟩ := tr_inj h h₁; rfl
+
+theorem State.aSimPairs_point_eq_of_state_eq {s : State} {s₁ p₁ p₂ st} [hs : sys.WF s]
+(h₁ : (s₁, p₁) ∈ s.aSimPairs st) (h₂ : (s₁, p₂) ∈ s.aSimPairs st) : p₁ = p₂ := by
+  rw [mem_aSimPairs_iff_simulate_tr] at h₁ h₂; grind
+
+@[simp]
+theorem State.aSimPtsNcard_empty {s : State} {st} : s.aSimPtsNcard st ∅ = some 0 := by
+  simp [aSimPtsNcard]
+
+@[simp]
+theorem State.aSimPtsNcard_eq_zero_iff {s : State} {st set} [hs : sys.WF s] :
+s.aSimPtsNcard st set = some 0 ↔ ∀ n s₁ s₂ [AState s₁],
+sys.simulate st.f s n = (s₁, 0) → sys.tr s₁ (st.a.f s₁) = some s₂ → s₂.aPos ∉ set := by
+  rw [aSimPtsNcard, Set.ncard?]
+  split_ifs with h₁; rotate_left
+  · simp at h₁ ⊢
+    replace h₁ := Set.exi_mem_of_infinite h₁
+    rcases h₁ with ⟨⟨s₁, p⟩, h₁⟩
+    simp at h₁
+    rw [mem_aSimPairs_iff_simulate_tr] at h₁
+    obtain ⟨⟨hs₁, n, h₁, s₂, h₂, h₃⟩, h₄⟩ := h₁
+    use n, s₁, hs₁, h₁, s₂, h₂
+    rwa [AState.aPos_eq_of_tr h₂, h₃]
+  simp
+  rw [Set.ncard_eq_zero # by grind]
+  rw [Set.eq_empty_iff]
+  simp
+  constructor
+  · intro h n s₁ s₂ hs₁ h₂ h₃
+    specialize h s₁ (st.a.f s₁)
+    rw [mem_aSimPairs_iff_simulate_tr] at h
+    rw [AState.aPos_eq_of_tr h₃]
+    apply h; clear h
+    use hs₁, n, h₂, s₂
+  · intro h s₁ p h₂
+    rw [mem_aSimPairs_iff_simulate_tr] at h₂
+    choose hs₁ n h₂ s₂ h₃ h₄ using h₂
+    specialize h n s₁ s₂ h₂ h₃
+    rwa [←h₄, ←AState.aPos_eq_of_tr h₃]
+
+theorem State.aSimPairs_eq_of_length_hist_eq {s s₁ s₂ p₁ p₂ st} [hs : sys.WF s]
+(h₁ : (s₁, p₁) ∈ s.aSimPairs st) (h₂ : (s₂, p₂) ∈ s.aSimPairs st)
+(h₃ : s₁.hist.length = s₂.hist.length) : s₁ = s₂ := by
+  rw [mem_aSimPairs_iff_simulate_tr] at h₁ h₂
+  choose hs₁ n h₁ h₄ h₅ h₆ using h₁
+  choose hs₂ k h₂ h₇ h₈ h₉ using h₂
+  simp [length_hist_eq_of_simulate_eq h₁, length_hist_eq_of_simulate_eq h₂] at h₃
+  subst h₃
+  simp [h₁] at h₂
+  exact h₂
+
+theorem State.finite_filter_aSimPairs_iff_image_length_hist {s : State} {st p}
+[hs : sys.WF s] : (s.aSimPairs st |>.filter p |>.Finite) ↔
+(s.aSimPairs st |>.filter p |>.image (·.1.hist.length) |>.Finite) := by
+  rw [Set.finite_image_iff]
+  rintro ⟨s₂, p₂⟩ h₄ ⟨s₃, p₃⟩ h₅ h₆
+  simp at h₄ h₅ h₆ ⊢
+  rcases h₄ with ⟨h₄, hp₂⟩
+  rcases h₅ with ⟨h₅, hp₃⟩
+  apply and_of # aSimPairs_eq_of_length_hist_eq h₄ h₅ h₆
+  rintro rfl; exact aSimPairs_point_eq_of_state_eq h₄ h₅
+
+theorem State.infinite_filter_aSimPairs_iff_image_length_hist {s : State} {st p}
+[hs : sys.WF s] : (s.aSimPairs st |>.filter p |>.Infinite) ↔
+(s.aSimPairs st |>.filter p |>.image (·.1.hist.length) |>.Infinite) := by
+  rw [iff_iff_not']; simp [finite_filter_aSimPairs_iff_image_length_hist]
+
+theorem State.nonempty_filter_aSimPairs_iff_image_length_hist {s : State} {st p} :
+(s.aSimPairs st |>.filter p |>.Nonempty) ↔
+(s.aSimPairs st |>.filter p |>.image (·.1.hist.length) |>.Nonempty) := by
+  simp
+
+theorem State.eq_simulate_eq_and_length_hist_eq {s s₁ s₂ n₁ n₂} {st : Strat}
+(h₁ : sys.simulate st.f s n₁ = (s₁, 0)) (h₂ : sys.simulate st.f s n₂ = (s₂, 0))
+(h₃ : s₁.hist.length = s₂.hist.length) : s₁ = s₂ := by
+  simp [length_hist_eq_of_simulate_eq h₁, length_hist_eq_of_simulate_eq h₂] at h₃
+  subst h₃; simp [h₁] at h₂; exact h₂
+
+theorem State.eq_of_mem_aSimPairs' {s st s₁ s₂ p₁ p₂} [hs : sys.WF s]
+(h₁ : (s₁, p₁) ∈ s.aSimPairs st) (h₂ : (s₂, p₂) ∈ s.aSimPairs st)
+(h₃ : s₁.hist.length = s₂.hist.length) : s₁ = s₂ ∧ p₁ = p₂ := by
+  rw [mem_aSimPairs_iff_simulate_tr] at h₁ h₂
+  choose hs₁ n₁ h₁ s₃ h₄ h₅ using h₁
+  choose hs₂ n₂ h₂ s₄ h₆ h₇ using h₂
+  apply and_of
+  · exact eq_simulate_eq_and_length_hist_eq h₁ h₂ h₃
+  rintro rfl
+  rw [←h₅, ←h₇]
+
+theorem State.eq_of_mem_aSimPairs {s st r₁ r₂} [hs : sys.WF s]
+(h₁ : r₁ ∈ s.aSimPairs st) (h₂ : r₂ ∈ s.aSimPairs st)
+(h₃ : r₁.1.hist.length = r₂.1.hist.length) : r₁ = r₂ := by
+  cases r₁; cases r₂; simp; exact eq_of_mem_aSimPairs' h₁ h₂ h₃
+
+theorem State.ncard_filter_aSimPairs_eq_image_length_hist {s : State} {st p} [hs : sys.WF s] :
+(s.aSimPairs st |>.filter p |>.ncard) =
+(s.aSimPairs st |>.filter p |>.image (·.1.hist.length) |>.ncard) := by
+  rw [Set.ncard_eq_ite]
+  nth_rw 2 [Set.ncard_eq_ite]
+  rw [finite_filter_aSimPairs_iff_image_length_hist]
+  split_ifs with h
+  on_goal 2 => rfl
+  symm; rw [Set.ncard_image_eq_iff_injOn]
+  rotate_left; rwa [finite_filter_aSimPairs_iff_image_length_hist]
+  rintro ⟨s₁, p₁⟩ h₁ ⟨s₂, p₂⟩ h₂ h₃
+  simp at h₁ h₂ h₃
+  exact eq_of_mem_aSimPairs h₁.1 h₂.1 h₃
+
+theorem AState.aSeek_exi_tr_of {s P} [hs : AState s]
+(h : ∃ p s₁, sys.tr s p = some s₁ ∧ P s₁) :
+∃ s₁, sys.tr s (aSeek P |>.f s) = some s₁ ∧ P s₁ := by
+  simp [aSeek]
+  rw [choose?_eq_of_exi]
+  rotate_left; exact h
+  simp
+  have h₁ := Classical.epsilon_spec h
+  generalize hp : Classical.epsilon (λ p => ∃ s₁, sys.tr s p = some s₁ ∧ P s₁) = p at h₁ ⊢
+  choose s₁ h₁ h₂ using h₁
+  simpa [sys.validTr_of_eq_some h₁, h₁]
+
+theorem AState.ne_of_tr {s s₁ p} [hs : AState s]
+(h : sys.tr s p = some s₁) : p ≠ s.aPos := by
+  rw [tr_eq_some_iff] at h; grind
+
+theorem AState.aPos_ne_of_tr {s s₁ p} [hs : AState s]
+(h : sys.tr s p = some s₁) : s₁.aPos ≠ s.aPos := by
+  rw [tr_eq_some_iff] at h; grind
+
+theorem AState.exi_dState_of_aSimPtsNcard_eq_succ
+{s : State} {st : Strat} {set n} [hs : AState s] [hst : st.WF]
+(h : s.aSimPtsNcard st set = some (n + 1)) : ∃ n s₁,
+sys.simulate st.f s (n * 2 + 1) = (s₁, 0) ∧ s₁.aPos ∈ set ∧ ∀ k s₂, 2 ≤ k →
+sys.simulate st.f s₁ k = (s₂, 0) → s₂.aPos ∉ set := by
+  rw [State.aSimPtsNcard, Set.ncard?] at h; split_ifs at h with h₁
+  simp at h ⊢
+  replace h := congrArg (· = 0) h; simp at h
+  replace h := Set.nonempty_of_ncard_ne_zero h
+  rw [State.finite_filter_aSimPairs_iff_image_length_hist] at h₁
+  rw [State.nonempty_filter_aSimPairs_iff_image_length_hist] at h
+  have h₂ := Set.exi_max h₁ h
+  clear h₁ h n
+  simp only [Set.mem_image, Set.mem_filter, Prod.exists, exists_and_right, forall_exists_index,
+    and_imp, exists_exists_and_eq_and] at h₂
+  obtain ⟨s₁, ⟨p, h₁, h₂⟩, h₃⟩ := h₂
+  rw [State.mem_aSimPairs_iff_simulate_tr] at h₁
+  rcases h₁ with ⟨hs₁, n, h₁, s₂, h₄, rfl⟩
+  have hs₂ := DState.of_tr h₄
+  obtain ⟨n, rfl⟩ := Nat.even_iff_exi.mp # even_of_simulate h₁
+  obtain ⟨s₃, h₅⟩ := st.d.validTr s₂
+  have hs₃ := AState.of_tr h₅
+  use n, s₂
+  simp [h₁, h₄]
+  split_ands
+  · rwa [AState.aPos_eq_of_tr h₄]
+  intro k s' hk h₆
+  iterate 2 cases k; simp at hk; nm k
+  clear hk
+  have hs' : sys.WF s'; grind
+  simp at h₆
+  obtain ⟨sd, ⟨sa, H₁, H₂⟩, H₃⟩ := h₆
+  have hsa : sys.WF sa; grind
+  have hsd : sys.WF sd; grind
+  replace hs' := s'.aState_or_dState; rcases hs' with hs' | hs'
+  · replace hsd : DState sd; grind
+    replace hsa : AState sa; grind
+    simp at H₂ H₃
+    specialize h₃ sa.hist.length sa (st.a.f sa) _
+    · rw [State.mem_aSimPairs_iff_simulate_tr]
+      use hsa, n * 2 + 1 + k
+      simp [*]
+    contrapose! h₃
+    simp
+    split_ands
+    · rw [DState.aPos_eq_of_tr H₃, AState.aPos_eq_of_tr H₂] at h₃
+      exact h₃
+    rw [State.length_hist_eq_of_simulate_eq H₁, length_hist_eq_of_tr h₄]
+    omega
+  · rename' sa => sd, sd => sa, hsa => hsd, hsd => hsa
+    replace hsa : AState sa; grind
+    replace hsd : DState sd; grind
+    simp at H₂ H₃
+    specialize h₃ sa.hist.length sa (st.a.f sa) _
+    · rw [State.mem_aSimPairs_iff_simulate_tr]
+      use hsa, n * 2 + 1 + k + 1
+      simp [*]
+    contrapose! h₃
+    simp
+    split_ands
+    · rwa [←AState.aPos_eq_of_tr H₃]
+    rw [length_hist_eq_of_tr H₂, State.length_hist_eq_of_simulate_eq H₁, length_hist_eq_of_tr h₄]
+    omega
+
+theorem AState.exi_aState_of_aSimPtsNcard_eq_succ
+{s : State} {st : Strat} {set n} [hs : AState s] [hst : st.WF]
+(h : s.aSimPtsNcard st set = some (n + 1)) : ∃ n s₁,
+sys.simulate st.f s (n * 2) = (s₁, 0) ∧ s₁.aPos ∈ set ∧ ∀ k s₂, k ≠ 0 →
+sys.simulate st.f s₁ k = (s₂, 0) → s₂.aPos ∉ set := by
+  choose k s₁ h₁ h₂ h₃ using exi_dState_of_aSimPtsNcard_eq_succ h
+  use k + 1
+  simp at h₁
+  choose s' h₁ h₄ using h₁
+  have hs' := AState.of_simulate_mul_two_eq_full h₁
+  have hs₁ := DState.of_tr h₄
+  simp at h₄
+  obtain ⟨s₂, h₅⟩ : sys.validTr s₁ # st.d.f s₁; simp
+  use s₂
+  simp_rw [Nat.add_mul]
+  simp [h₁, h₄, h₅, DState.aPos_eq_of_tr h₅, h₂]
+  intro r s₃ hr h₆
+  apply h₃ (r + 1) s₃ (by omega)
+  rw [sys.simulate_succ_full']
+  simpa [h₅]
+
+theorem AState.getd_aSimPtsNcard_lt_of_odd {s st₁ st₂ set} (n : ℕ)
+[hs : AState s] (hn : Odd n) (h₁ : s.aWins st₁) (h₂ : s.aWins st₂)
+(h₃ : s.aSimPtsNcard st₁ set |>.isSome) (h₄ : s.aSimPtsNcard st₂ set |>.isSome)
+(h₅ : ∀ k s₁ s₂, sys.simulate st₁.f s k = (s₁, 0) → sys.simulate st₂.f s k = (s₂, 0) →
+s₁.aPos ∈ set → s₂.aPos ∈ set) (h₆ : ∀ s₁, sys.simulate st₁.f s n = (s₁, 0) → s₁.aPos ∉ set)
+(h₇ : ∀ s₁, sys.simulate st₂.f s n = (s₁, 0) → s₁.aPos ∈ set) :
+(s.aSimPtsNcard st₁ set).getd < (s.aSimPtsNcard st₂ set).getd := by
+  obtain ⟨n, rfl⟩ := Nat.odd_iff_exi.mp hn; clear hn
+  rw [Option.isSome_iff_exists] at h₃ h₄
+  rcases h₃, h₄ with ⟨⟨N₁, h₃⟩, ⟨N₂, h₄⟩⟩
+  simp [h₃, h₄, Option.getd]
+  simp [State.aSimPtsNcard, Set.ncard?] at h₃ h₄
+  rcases h₃ with ⟨H₁, rfl⟩
+  rcases h₄ with ⟨H₃, rfl⟩
+  rw [State.finite_filter_aSimPairs_iff_image_length_hist] at H₁ H₃
+  simp_rw [State.ncard_filter_aSimPairs_eq_image_length_hist]
+  apply Set.ncard_lt_ncard _ H₃
+  clear H₁ H₃
+  replace h₆ : ∃ sd₁, sys.simulate st₁.f s (n * 2 + 1) = (sd₁, 0) ∧ sd₁.aPos ∉ set
+  · specialize h₁ (n * 2 + 1); grind
+  replace h₇ : ∃ sd₂, sys.simulate st₂.f s (n * 2 + 1) = (sd₂, 0) ∧ sd₂.aPos ∈ set
+  · specialize h₂ (n * 2 + 1); grind
+  choose sd₁ G₁ G₂ using h₆
+  choose sd₂ G₃ G₄ using h₇
+  simp at G₁ G₃
+  choose sa₁ G₁ G₅ using G₁
+  choose sa₂ G₃ G₆ using G₃
+  have hsa₁ := AState.of_simulate_mul_two_eq_full G₁
+  have hsa₂ := AState.of_simulate_mul_two_eq_full G₃
+  have hsd₁ := DState.of_tr G₅
+  have hsd₂ := DState.of_tr G₆
+  simp at G₅ G₆
+  apply Set.ssubset_of # s.hist.length + n * 2
+  · intro k hk
+    simp at hk ⊢
+    obtain ⟨s₁, ⟨p, H₁, H₂⟩, hk⟩ := hk
+    have h₂' := h₂
+    specialize h₂ (k - s.hist.length)
+    generalize hr : sys.simulate st₂.f s (k - s.hist.length) = r
+    rcases r with ⟨s₁', r⟩
+    simp [hr] at h₂; subst h₂
+    rw [State.mem_aSimPairs_iff_simulate_tr] at H₁
+    choose hs₁ c H₁ H₃ using H₁
+    simp [State.length_hist_eq_of_simulate_eq H₁] at hk
+    subst hk
+    simp at hr
+    obtain ⟨s₂, H₃, rfl⟩ := H₃
+    have hs₁' : AState s₁'
+    · obtain ⟨c, rfl⟩ := Nat.even_iff_exi.mp # AState.even_of_simulate H₁
+      exact AState.of_simulate_mul_two_eq_full hr
+    specialize h₂' (c + 1)
+    simp [hr] at h₂'
+    choose s₂' H₄ using h₂'
+    refine ⟨s₁', ⟨st₂.f s₁', ?_, ?_⟩, ?_⟩
+    · rw [State.mem_aSimPairs_iff_simulate_tr]
+      use hs₁'
+      use c, hr, s₂', H₄
+      simp
+    · simp
+      rw [←AState.aPos_eq_of_tr H₄]
+      specialize h₅ (c + 1)
+      simp [H₁, hr, H₃, H₄] at h₅
+      apply h₅
+      rwa [AState.aPos_eq_of_tr H₃]
+    · simp [State.length_hist_eq_of_simulate_eq hr]
+  · simp
+    intro S p H₁ H₂ H₃
+    rw [State.mem_aSimPairs_iff_simulate_tr] at H₁
+    choose hS k H₁ S' H₄ H₅ using H₁
+    subst H₅
+    simp [State.length_hist_eq_of_simulate_eq H₁] at H₃
+    subst H₃
+    simp [G₁] at H₁
+    subst H₁
+    simp [AState.aPos_eq_of_tr G₅, H₂] at G₂
+  · simp
+    refine ⟨sa₂, ⟨st₂.a.f sa₂, ?_, ?_⟩, ?_⟩
+    · rw [State.mem_aSimPairs_iff_simulate_tr]
+      use hsa₂, n * 2, G₃
+      simp [G₆]
+    · rwa [←AState.aPos_eq_of_tr G₆]
+    · rw [State.length_hist_eq_of_simulate_eq G₃]
+
+theorem AState.getd_aSimPtsNcard_lt_of {s st₁ st₂ set} (n : ℕ)
+[hs : AState s] (h₁ : s.aWins st₁) (h₂ : s.aWins st₂)
+(h₃ : s.aSimPtsNcard st₁ set |>.isSome) (h₄ : s.aSimPtsNcard st₂ set |>.isSome)
+(h₅ : ∀ k s₁ s₂, sys.simulate st₁.f s k = (s₁, 0) → sys.simulate st₂.f s k = (s₂, 0) →
+s₁.aPos ∈ set → s₂.aPos ∈ set) (h₆ : ∀ s₁, sys.simulate st₁.f s n = (s₁, 0) → s₁.aPos ∉ set)
+(h₇ : ∀ s₁, sys.simulate st₂.f s n = (s₁, 0) → s₁.aPos ∈ set) :
+(s.aSimPtsNcard st₁ set).getd < (s.aSimPtsNcard st₂ set).getd := by
+  induction n using Nat.mod_2_ind <;> nm n
+  rotate_left
+  · apply getd_aSimPtsNcard_lt_of_odd (n * 2 + 1) <;> try assumption;; simp
+  generalize hk : n * 2 - 1 = k
+  replace hk : n * 2 = k + 1
+  · cases n
+    · simp at h₆ h₇; contradiction
+    nm n; omega
+  rw [hk] at h₆ h₇
+  obtain ⟨m, hm⟩ : ∃ m, k = m * 2 + 1
+  · rw [←Nat.odd_iff_exi, Nat.odd_iff]; omega
+  apply getd_aSimPtsNcard_lt_of_odd k <;> try assumption
+  · simp [hm]
+  · intro s₁ H₁
+    specialize h₁ (k + 1)
+    simp [H₁] at h₁
+    choose s₂ h₁ using h₁
+    rw [hm] at H₁
+    have hs₁ := DState.of_simulate_mul_two_add_one_eq_full H₁
+    rw [←DState.aPos_eq_of_tr h₁]
+    apply h₆
+    rw [←hm] at H₁
+    simp at h₁
+    simpa [H₁]
+  · intro s₁ H₁
+    specialize h₂ (k + 1)
+    simp [H₁] at h₂
+    choose s₂ h₂ using h₂
+    rw [hm] at H₁
+    have hs₁ := DState.of_simulate_mul_two_add_one_eq_full H₁
+    rw [←DState.aPos_eq_of_tr h₂]
+    apply h₇
+    rw [←hm] at H₁
+    simp at h₂
+    simpa [H₁]
+
+theorem State.validTr_of_mem_aSimPairs {s s' p st} [hs : sys.WF s]
+(h : (s', p) ∈ s.aSimPairs st) : sys.validTr s' p := by
+  rw [mem_aSimPairs_iff_simulate_tr] at h; rw [sys.validTr_iff_isSome]; grind
+
+theorem steps_eq_of_simulate_full_eq {s s₁ n m f} [hs : sys.WF s]
+(h₁ : sys.simulate f s n = (s₁, 0)) (h₂ : sys.simulate f s m = (s₁, 0)) : n = m := by
+  rw [←length_hist_sub_eq_of_simulate h₁, length_hist_sub_eq_of_simulate h₂]
+
+theorem State.mem_simStatesRangeAuxVia_iff {s s₁ s' : State} {st r n} [hr : DecidableRel r]
+(h : sys.simulate st.f s n = (s₁, 0)) : s' ∈ s.simStatesRangeAuxVia r st s₁ ↔
+s' ∈ s.simStates st ∧ s' ∈ (s.simStates st |>.filter (λ s₃ =>
+s₃.hist.length ≤ s₁.hist.length ∧ r s₃.hist.length s₁.hist.length)) := by
+  have h' : ∃ n, sys.simulate st.f s n = (s₁, 0) := ⟨_, h⟩
+  simp [simStatesRangeAuxVia, ReachableVia, ReachableVia', h', diff_eq_of_simulate_full h]
+  constructor
+  · rintro ⟨⟨k, hk, h₂⟩, h₃⟩
+    generalize hc : sys.simulate st.f s k = c at h₂
+    rcases c with ⟨s', c⟩; simp at h₂; subst h₂
+    obtain ⟨n, rfl⟩ := Nat.exists_eq_add_of_le hk; clear hk
+    simp [hc] at h
+    rcases h with ⟨rfl, h⟩
+    split_ands
+    · use k
+    · apply length_hist_le_of_reachable
+      exact sys.reachable_of_simulate h
+    · exact h₃
+  · rintro ⟨⟨k, h₁⟩, h₂, h₃⟩
+    simp [h₃]
+    use k
+    simp [h₁]
+    have := length_hist_eq_of_simulate_eq h
+    have := length_hist_eq_of_simulate_eq h₁
+    omega
+
+theorem State.mem_simStatesIccVia_iff_of {s s₁ s₂ : State} {st : Strat} {n}
+(h : sys.simulate st.f s n = (s₁, 0)) : s₂ ∈ s.simStatesIccVia st s₁ ↔
+∃ k, k ≤ n ∧ sys.simulate st.f s k = (s₂, 0) := by
+  simp [simStatesIccVia, mem_simStatesRangeAuxVia_iff h]; constructor
+  · rintro ⟨⟨k, h₁⟩, h₂⟩; use k; simp [h₁]; have := length_hist_eq_of_simulate_eq h
+    have := length_hist_eq_of_simulate_eq h₁; omega
+  · rintro ⟨k, h₁, h₂⟩; use by use k;; have := length_hist_eq_of_simulate_eq h
+    have := length_hist_eq_of_simulate_eq h₂; omega
+
+theorem State.mem_simStatesIcoVia_iff_of {s s₁ s₂ : State} {st : Strat} {n}
+(h : sys.simulate st.f s n = (s₁, 0)) : s₂ ∈ s.simStatesIcoVia st s₁ ↔
+∃ k, k < n ∧ sys.simulate st.f s k = (s₂, 0) := by
+  simp [simStatesIcoVia, ReachableVia, mem_simStatesRangeAuxVia_iff h]; constructor
+  · rintro ⟨⟨k, h₁⟩, h₂⟩; use k; simp [h₁]; have := length_hist_eq_of_simulate_eq h
+    have := length_hist_eq_of_simulate_eq h₁; omega
+  · rintro ⟨k, h₁, h₂⟩; use by use k;; have := length_hist_eq_of_simulate_eq h
+    have := length_hist_eq_of_simulate_eq h₂; omega
+
+theorem State.mem_aSimStatesIccVia_iff_of {s s₁ s₂ : State} {st : Strat} {n} [hs : sys.WF s]
+(h : sys.simulate st.f s n = (s₁, 0)) : s₂ ∈ s.aSimStatesIccVia st s₁ ↔ AState s₂ ∧
+∃ k, k ≤ n ∧ sys.simulate st.f s k = (s₂, 0) := by
+  simp [aSimStatesIccVia, mem_simStatesIccVia_iff_of h]
+  rw [and_comm]; constructor
+  · rintro ⟨h₁, k, hk, h₂⟩
+    have hs₂ : sys.WF s₂; grind
+    rw [aTurn_iff_aState] at h₁; tauto
+  · rintro ⟨h₁, k, hk, h₂⟩; simp; tauto
+
+theorem State.mem_aSimStatesIcoVia_iff_of {s s₁ s₂ : State} {st : Strat} {n} [hs : sys.WF s]
+(h : sys.simulate st.f s n = (s₁, 0)) : s₂ ∈ s.aSimStatesIcoVia st s₁ ↔ AState s₂ ∧
+∃ k, k < n ∧ sys.simulate st.f s k = (s₂, 0) := by
+  simp [aSimStatesIcoVia, mem_simStatesIcoVia_iff_of h]
+  rw [and_comm]; constructor
+  · rintro ⟨h₁, k, hk, h₂⟩
+    have hs₂ : sys.WF s₂; grind
+    rw [aTurn_iff_aState] at h₁; tauto
+  · rintro ⟨h₁, k, hk, h₂⟩; simp; tauto
+
+theorem State.mem_simStatesIccVia_iff {s s₁ s₂ : State} {st : Strat} [hs : sys.WF s] :
+s₁ ∈ s.simStatesIccVia st s₂ ↔ ∃ k n, k ≤ n ∧ sys.simulate st.f s k = (s₁, 0) ∧
+sys.simulate st.f s n = (s₂, 0) := by
+  by_cases h₁ : ∃ n, sys.simulate st.f s n = (s₂, 0)
+  · choose n h₁ using h₁
+    rw [mem_simStatesIccVia_iff_of h₁]
+    constructor
+    · rintro ⟨k, hk, h₂⟩
+      use k, n
+    · rintro ⟨k, n', hk, h₂, h₃⟩
+      cases steps_eq_of_simulate_full_eq h₁ h₃
+      use k
+  · simp [simStatesIccVia, simStatesRangeAuxVia, ReachableVia, ReachableVia', h₁]
+    push_neg at h₁
+    intro k n hk h₂
+    apply h₁
+
+theorem State.mem_simStatesIcoVia_iff {s s₁ s₂ : State} {st : Strat} [hs : sys.WF s] :
+s₁ ∈ s.simStatesIcoVia st s₂ ↔ ∃ k n, k < n ∧ sys.simulate st.f s k = (s₁, 0) ∧
+sys.simulate st.f s n = (s₂, 0) := by
+  by_cases h₁ : ∃ n, sys.simulate st.f s n = (s₂, 0)
+  · choose n h₁ using h₁
+    rw [mem_simStatesIcoVia_iff_of h₁]
+    constructor
+    · rintro ⟨k, hk, h₂⟩
+      use k, n
+    · rintro ⟨k, n', hk, h₂, h₃⟩
+      cases steps_eq_of_simulate_full_eq h₁ h₃
+      use k
+  · simp [simStatesIcoVia, simStatesRangeAuxVia, ReachableVia, ReachableVia', h₁]
+    push_neg at h₁
+    intro k n hk h₂
+    apply h₁
+
+theorem State.mem_aSimStatesIccVia_iff {s s₁ s₂ : State} {st : Strat} [hs : sys.WF s] :
+s₁ ∈ s.aSimStatesIccVia st s₂ ↔ AState s₁ ∧ ∃ k n, k ≤ n ∧ sys.simulate st.f s k = (s₁, 0) ∧
+sys.simulate st.f s n = (s₂, 0) := by
+  simp [aSimStatesIccVia, mem_simStatesIccVia_iff]; rw [and_comm]; constructor
+  · rintro ⟨ht, k, n, hk, h₁, h₂⟩; have hs₁ : sys.WF s₁; grind
+    rw [aTurn_iff_aState] at ht; use ht, k, n
+  · rintro ⟨hs₁, h⟩; simpa
+
+theorem State.mem_aSimStatesIcoVia_iff {s s₁ s₂ : State} {st : Strat} [hs : sys.WF s] :
+s₁ ∈ s.aSimStatesIcoVia st s₂ ↔ AState s₁ ∧ ∃ k n, k < n ∧ sys.simulate st.f s k = (s₁, 0) ∧
+sys.simulate st.f s n = (s₂, 0) := by
+  simp [aSimStatesIcoVia, mem_simStatesIcoVia_iff]; rw [and_comm]; constructor
+  · rintro ⟨ht, k, n, hk, h₁, h₂⟩; have hs₁ : sys.WF s₁; grind
+    rw [aTurn_iff_aState] at ht; use ht, k, n
+  · rintro ⟨hs₁, h⟩; simpa
+
+@[simp]
+theorem State.simulate_full_eq_self_iff {s : State} {f n} :
+sys.simulate f s n = (s, 0) ↔ n = 0 := by
+  symm; constructor; rintro ⟨rfl, rfl⟩; simp
+  intro h; have := length_hist_eq_of_simulate_eq h; omega
+
+@[simp]
+theorem State.mem_simStatesIccVia_self_iff {s s' : State} {st} [hs : sys.WF s] :
+s' ∈ s.simStatesIccVia st s ↔ s' = s := by
+  simp [mem_simStatesIccVia_iff]
+
+theorem State.exi_aPos_simulate_eq_of_aPos_simulate_ne {s s₁ : State} {f n}
+[hs : sys.WF s] (h₁ : sys.simulate f s n = (s₁, 0)) (h₂ : s₁.aPos ≠ s.aPos) :
+∃ k < n, ∃ s₀ s', AState s₀ ∧ DState s' ∧ sys.simulate f s k = (s₀, 0) ∧
+sys.tr s₀ (f s₀) = some s' ∧ s'.aPos = s₁.aPos := by
+  induction n generalizing s₁
+  · simp at h₁; simp [h₁] at h₂
+  nm n ih; rename' s₁ => s₂; simp at h₁; rcases h₁ with ⟨s₁, h₁, h₃⟩
+  have hs₁ : sys.WF s₁; grind; replace hs₁ := s₁.aState_or_dState
+  rcases hs₁ with hs₁ | hs₁
+  · have hs₂ := DState.of_tr h₃; use n, by simp, s₁, s₂
+  · specialize ih h₁; rw [DState.aPos_eq_of_tr h₃] at h₂ ⊢
+    specialize ih h₂; choose k hk s₀ s' hs₀ hs' h₄ h₅ h₆ using ih
+    use k, by omega, s₀, s'
+
+theorem State.mem_aVisitedIcc_of_mem_simStatesIccVia {s s' s₁ : State} {st : Strat} {n}
+[hs : sys.WF s] (h₁ : sys.simulate st.f s n = (s₁, 0))
+(h₂ : s' ∈ s.simStatesIccVia st s₁) : s'.aPos ∈ s.aVisitedIcc s₁ := by
+  rw [mem_simStatesIccVia_iff_of h₁] at h₂; choose k hk h₂ using h₂
+  rw [mem_aVisitedIcc_iff_of h₁, or_iff_not_imp_left]; intro h₃
+  choose r hr s₀ s₂ hs₀ hs₂ h₄ h₅ h₆ using exi_aPos_simulate_eq_of_aPos_simulate_ne h₂ h₃
+  use r, by omega, s₀, hs₀, h₄; rwa [←AState.aPos_eq_of_tr h₅]
+
+theorem State.mem_aVisitedIcc_iff_mem_simStatesIccVia {s s₁ : State} {st : Strat} {n p}
+[hs : sys.WF s] (h : sys.simulate st.f s n = (s₁, 0)) :
+p ∈ s.aVisitedIcc s₁ ↔ ∃ s' ∈ s.simStatesIccVia st s₁, s'.aPos = p := by
+  symm; constructor; rintro ⟨s', h₁, rfl⟩; exact mem_aVisitedIcc_of_mem_simStatesIccVia h h₁
+  rw [mem_aVisitedIcc_iff_of h]; intro h₁; simp [mem_simStatesIccVia_iff]
+  rcases h₁ with (rfl | ⟨k, hk, s', hs', h₁, rfl⟩); use s; simp; use n
+  replace hk : ∃ r, k + 1 + r = n; use n - k - 1; omega
+  obtain ⟨n, rfl⟩ := hk; simp [h₁] at h; choose s' h h₂ using h
+  nm s₀; simp [←AState.aPos_eq_of_tr h]; use s'
+  simp; use k + 1, k + 1 + n, by omega;; simpa [h₁, h]
+
+theorem State.mem_simStatesIccVia_of_mem_simStatesIcoVia {s s₁ s' : State} {st} [hs : sys.WF s]
+(h : s' ∈ s.simStatesIcoVia st s₁) : s' ∈ s.simStatesIccVia st s₁ := by
+  rw [mem_simStatesIcoVia_iff] at h; rw [mem_simStatesIccVia_iff]
+  choose k n hk h₁ h₂ using h; use k, n, by omega
+
+theorem State.mem_aSimStatesIccVia_of_mem_aSimStatesIcoVia {s s₁ s' : State} {st} [hs : sys.WF s]
+(h : s' ∈ s.aSimStatesIcoVia st s₁) : s' ∈ s.aSimStatesIccVia st s₁ := by
+  rw [mem_aSimStatesIcoVia_iff] at h; rw [mem_aSimStatesIccVia_iff]
+  choose hs' k n hk h₁ h₂ using h; use hs', k, n, by omega
+
+theorem State.simStatesIcoVia_subset_simStatesIccVia {s s₁ : State} {st} [hs : sys.WF s] :
+s.simStatesIcoVia st s₁ ⊆ s.simStatesIccVia st s₁ :=
+  λ _ => mem_simStatesIccVia_of_mem_simStatesIcoVia
+
+theorem State.aSimStatesIcoVia_subset_aSimStatesIccVia {s s₁ : State} {st} [hs : sys.WF s] :
+s.aSimStatesIcoVia st s₁ ⊆ s.aSimStatesIccVia st s₁ :=
+  λ _ => mem_aSimStatesIccVia_of_mem_aSimStatesIcoVia
+
+theorem State.simStatesIcoVia_eq_erase_simStatesIccVia {s s₁ : State} {st} [hs : sys.WF s] :
+s.simStatesIcoVia st s₁ = (s.simStatesIccVia st s₁).erase s₁ := by
+  ext s'; simp [mem_simStatesIcoVia_iff, mem_simStatesIccVia_iff]; constructor
+  · rintro ⟨k, n, hk, h₁, h₂⟩
+    symm; split_ands; use k, n, by omega
+    rintro rfl
+    simp [steps_eq_of_simulate_full_eq h₁ h₂] at hk
+  · rintro ⟨h, k, n, hk, h₁, h₂⟩
+    use k, n
+    split_ands <;> try assumption
+    contrapose! h
+    replace h : n = k; omega
+    simp [h, h₁] at h₂
+    exact h₂
+
+theorem State.aSimStatesIcoVia_eq_erase_aSimStatesIccVia {s s₁ : State} {st} [hs : sys.WF s] :
+s.aSimStatesIcoVia st s₁ = (s.aSimStatesIccVia st s₁).erase s₁ := by
+  unfold aSimStatesIcoVia aSimStatesIccVia
+  rw [simStatesIcoVia_eq_erase_simStatesIccVia]
+  ext; simp; tauto
+
+theorem State.mem_simStatesIcoVia_mem_simStatesIccVia_and_ne {s s₁ s' : State} {st} [hs : sys.WF s]
+(h₁ : s' ∈ s.simStatesIccVia st s₁) (h₂ : s' ≠ s₁) : s' ∈ s.simStatesIcoVia st s₁ := by
+  simp [simStatesIcoVia_eq_erase_simStatesIccVia]; tauto
+
+theorem State.mem_aSimStatesIcoVia_of_mem_aSimStatesIccVia_and_ne
+{s s₁ s' : State} {st} [hs : sys.WF s]
+(h₁ : s' ∈ s.aSimStatesIccVia st s₁) (h₂ : s' ≠ s₁) : s' ∈ s.aSimStatesIcoVia st s₁ := by
+  simp [aSimStatesIcoVia_eq_erase_aSimStatesIccVia]; tauto
+
+theorem State.mem_simStatesIccVia_of_mem_aSimStatesIccVia {s s₁ s' : State} {st}
+(h : s' ∈ s.aSimStatesIccVia st s₁) : s' ∈ s.simStatesIccVia st s₁ := by
+  simp [aSimStatesIccVia] at h; exact h.1
+
+theorem State.mem_simStatesIcoVia_of_mem_aSimStatesIcoVia {s s₁ s' : State} {st}
+(h : s' ∈ s.aSimStatesIcoVia st s₁) : s' ∈ s.simStatesIcoVia st s₁ := by
+  simp [aSimStatesIcoVia] at h; exact h.1
+
+theorem State.mem_aVisitedIcc_of_mem_aSimStatesIccVia {s s' s₁ : State} {st : Strat} {n}
+[hs : sys.WF s] (h₁ : sys.simulate st.f s n = (s₁, 0))
+(h₂ : s' ∈ s.aSimStatesIccVia st s₁) : s'.aPos ∈ s.aVisitedIcc s₁ :=
+  mem_aVisitedIcc_of_mem_simStatesIccVia h₁ # mem_simStatesIccVia_of_mem_aSimStatesIccVia h₂
+
+theorem State.mem_aVisitedIcc_of_mem_aSimStatesIcoVia {s s' s₁ : State} {st : Strat} {n}
+[hs : sys.WF s] (h₁ : sys.simulate st.f s n = (s₁, 0))
+(h₂ : s' ∈ s.aSimStatesIcoVia st s₁) : s'.aPos ∈ s.aVisitedIcc s₁ :=
+  mem_aVisitedIcc_of_mem_aSimStatesIccVia h₁ # mem_aSimStatesIccVia_of_mem_aSimStatesIcoVia h₂
+
+theorem wf_of_mem_simStates {s s' : State} {st} [hs : sys.WF s]
+(h : s' ∈ s.simStates st) : sys.WF s' := by
+  rw [State.mem_simStates_iff] at h; choose n h using h; grind
+
+theorem wf_of_mem_simStatesRangeAuxVia {s s₁ s' : State} {st r}
+[hr : DecidableRel r] [hs : sys.WF s]
+(h : s' ∈ s.simStatesRangeAuxVia r st s₁) : sys.WF s' := by
+  simp [State.simStatesRangeAuxVia] at h; split_ifs at h with h₁ <;> simp at h
+  obtain ⟨⟨-, -, rfl⟩, -⟩ := h; infer_instance
+
+theorem wf_of_mem_simStatesIccVia {s s₁ s' : State} {st} [hs : sys.WF s]
+(h : s' ∈ s.simStatesIccVia st s₁) : sys.WF s' :=
+  wf_of_mem_simStatesRangeAuxVia h
+
+theorem wf_of_mem_simStatesIcoVia {s s₁ s' : State} {st} [hs : sys.WF s]
+(h : s' ∈ s.simStatesIcoVia st s₁) : sys.WF s' :=
+  wf_of_mem_simStatesRangeAuxVia h
+
+theorem State.mem_aVisitedIcc_iff_mem_aSimStatesIccVia {s s₁ : State} {st : Strat} {n p}
+[hs : sys.WF s] [hs₁ : AState s₁] (h : sys.simulate st.f s n = (s₁, 0)) :
+p ∈ s.aVisitedIcc s₁ ↔ ∃ s' ∈ s.aSimStatesIccVia st s₁, s'.aPos = p := by
+  symm; constructor; rintro ⟨s', h₂, rfl⟩; exact mem_aVisitedIcc_of_mem_aSimStatesIccVia h h₂
+  intro h₁
+  rw [mem_aVisitedIcc_iff_of h] at h₁
+  simp [mem_aSimStatesIccVia_iff]
+  simp [and_assoc]
+  rcases h₁ with (rfl | ⟨k, hk, s', hs', h₁, rfl⟩)
+  · replace hs := s.aState_or_dState
+    rcases hs with hs | hs
+    · use s
+      simp
+      use hs, n
+    cases n
+    · simp at h
+      subst h
+      cases s.false_of_aState_and_dState
+    nm n
+    rw [add_comm] at h
+    simp at h
+    choose s' h₁ h₃ using h
+    have hs' := AState.of_tr h₁
+    use s'
+    simp [hs', DState.aPos_eq_of_tr h₁]
+    use 1, 1 + n, by simp
+    simp; tauto
+  replace hk : ∃ r, k + 1 + r = n; use n - k - 1; omega
+  obtain ⟨n, rfl⟩ := hk; simp [h₁] at h; choose s' h h₂ using h
+  nm s₀; simp [←AState.aPos_eq_of_tr h]
+  cases n
+  · simp at h₂
+    subst h₂
+    have h₁ := DState.of_tr h
+    cases s'.false_of_aState_and_dState
+  nm n
+  rw [add_comm] at h₂
+  simp at h₂
+  choose s₂ h₂ h₃ using h₂
+  rename' hs' => hs₀
+  have hs' := sys.wf_of_tr h
+  replace hs' := s'.aState_or_dState
+  rcases hs' with hs' | hs'
+  · use s', hs'
+    simp
+    use k + 1, k + 2 + n, by omega
+    simp at h₂
+    simpa [h, h₁, h₂]
+  · have hs₂ := AState.of_tr h₂
+    use s₂, hs₂
+    simp [←DState.aPos_eq_of_tr h₂]
+    use k + 2, k + 2 + n, by omega
+    simp at h₂
+    simpa [h, h₁, h₂]
+
+theorem State.wf_prev_of_reachable_and_ne {s s₁ : State} [hs : sys.WF s]
+(h₁ : sys.Reachable s s₁) (h₂ : s ≠ s₁) : sys.WF s₁.prev := by
+  have hs₁ := sys.wf_of_reachable h₁
+  apply wf_prev
+  rw [System.reachable_iff_exi_trs] at h₁
+  choose ps h₁ using h₁
+  cases ps
+  · simp [h₂] at h₁
+  nm p ps
+  rw [isInit_iff_length_hist_eq_one]
+  rw [length_hist_eq_of_trs_eq h₁]
+  simp
+  suffices : s.hist.length ≠ 0; omega
+  simp
+
+theorem State.reachable_prev_of_reachable_and_ne {s s₁ : State} [hs : sys.WF s]
+(h₁ : sys.Reachable s s₁) (h₂ : s ≠ s₁) : sys.Reachable s s₁.prev := by
+  rw [System.reachable_iff_exi_trs] at h₁ ⊢
+  choose ps h₁ using h₁
+  induction ps using List.reverseRecOn
+  · simp [h₂] at h₁
+  nm ps p ih; clear ih
+  simp at h₁
+  choose s' h₁ h₃ using h₁
+  use ps
+  simp [h₁]
+  have hs' := sys.wf_of_trs h₁
+  rw [prev_eq_of_tr h₃]
+
+theorem State.mem_aVisitedIcc'_append {s : State} {ps₁ ps₂ p}
+(h : p ∈ s.aVisitedIcc' ps₁) : p ∈ s.aVisitedIcc' (ps₁ ++ ps₂) := by
+  induction ps₁ generalizing s
+  · simp at h
+  nm p₁ ps₁ ih
+  simp [aVisitedIcc'] at h ⊢
+  split_ifs at h ⊢ with h₁
+  · simp at h ⊢
+    rcases h with rfl | h
+    · left; rfl
+    right
+    exact ih h
+  exact ih h
+
+theorem State.mem_aVisitedIcc_of_mem_aVisitedIco {s s₁ : State} {p} [hs : sys.WF s]
+(h₁ : sys.Reachable s s₁) (h₂ : p ∈ s.aVisitedIco s₁) : p ∈ s.aVisitedIcc s₁ := by
+  rw [aVisitedIco] at h₂
+  split_ifs at h₂ with h₃
+  · simp at h₂
+  unfold aVisitedIcc at h₂ ⊢
+  simp [h₁]
+  have hs₁ := sys.wf_of_reachable h₁
+  have hsp := wf_prev_of_reachable_and_ne h₁ h₃
+  simp [reachable_prev_of_reachable_and_ne h₁ h₃] at h₂
+  rcases h₂ with rfl | h₂
+  · simp
+  right
+  rw [sys.reachable_iff_exi_trs] at h₁
+  choose ps h₁ using h₁
+  induction ps using List.reverseRecOn
+  · simp [h₃] at h₁
+  nm ps p₁ ih; clear ih
+  simp at h₁
+  choose s' h₁ h₄ using h₁
+  have hs' := sys.wf_of_trs h₁
+  rw [prev_eq_of_tr h₄] at h₂
+  rw [diffTrs_eq_of_tr h₄ # sys.reachable_of_trs h₁]
+  exact mem_aVisitedIcc'_append h₂
+
+set_option linter.unusedVariables false in
+theorem State.false_of_simulate_eq_simulate (s f s₁ s₂ n m) [hs : sys.WF s]
+(h₁ : sys.simulate f s n = (s₁, 0)) (h₂ : sys.simulate f s m = (s₁, 0))
+(h₃ : s₁ = s₂) (h₄ : n ≠ m) : False := by
+  subst h₃; exact h₄ # steps_eq_of_simulate_full_eq h₁ h₂
+
+theorem State.mem_aVisitedIco_iff_of {s f n s₁ p} [hs : sys.WF s]
+(h : sys.simulate f s n = (s₁, 0)) : p ∈ s.aVisitedIco s₁ ↔ (n ≠ 0 ∧ p = s.aPos) ∨
+∃ k, k + 1 < n ∧ ∃ s', AState s' ∧ sys.simulate f s k = (s', 0) ∧ f s' = p := by
+  unfold aVisitedIco
+  cases n
+  · simp at h
+    simp [h]
+  nm n
+  simp at h
+  choose s' h₁ h₂ using h
+  rw [if_neg]; rotate_left
+  · rintro rfl
+    apply s.false_of_simulate_eq_simulate f s s 0 (n + 1) <;> simp_all
+  have hs' : sys.WF s'; grind
+  rw [prev_eq_of_tr h₂, mem_aVisitedIcc_iff_of h₁]; grind
+
+theorem State.mem_aVisitedIco_of_mem_simStatesIcoVia {s s' s₁ : State} {st : Strat} {n}
+[hs : sys.WF s] (h₁ : sys.simulate st.f s n = (s₁, 0))
+(h₂ : s' ∈ s.simStatesIcoVia st s₁) : s'.aPos ∈ s.aVisitedIco s₁ := by
+  rw [mem_simStatesIcoVia_iff_of h₁] at h₂; choose k hk h₂ using h₂
+  rw [mem_aVisitedIco_iff_of h₁, or_iff_not_imp_left]; intro h₃
+  rw [not_and_iff_or] at h₃
+  simp at h₃
+  rcases h₃ with rfl | h₃
+  · simp at hk
+  choose r hr s₀ s₂ hs₀ hs₂ h₄ h₅ h₆ using exi_aPos_simulate_eq_of_aPos_simulate_ne h₂ h₃
+  use r, by omega, s₀, hs₀, h₄; rwa [←AState.aPos_eq_of_tr h₅]
+
+theorem State.mem_aVisitedIco_iff_mem_simStatesIcoVia {s s₁ : State} {st : Strat} {n p}
+[hs : sys.WF s] (h : sys.simulate st.f s n = (s₁, 0)) :
+p ∈ s.aVisitedIco s₁ ↔ ∃ s' ∈ s.simStatesIcoVia st s₁, s'.aPos = p := by
+  symm; constructor; rintro ⟨s', h₁, rfl⟩; exact mem_aVisitedIco_of_mem_simStatesIcoVia h h₁
+  rw [mem_aVisitedIco_iff_of h]; intro h₁; simp [mem_simStatesIcoVia_iff]
+  rcases h₁ with (⟨hn, rfl⟩ | ⟨k, hk, s', hs', h₁, rfl⟩)
+  · use s; simp; use n
+    simp [h]
+    omega
+  replace hk : ∃ r, k + 2 + r = n; use n - k - 2; omega
+  obtain ⟨n, rfl⟩ := hk; simp [h₁] at h; choose s' h h₂ using h
+  nm s₀
+  rename' hs' => hs₀
+  choose sx h h₃ using h
+  simp [←AState.aPos_eq_of_tr h]
+  use sx
+  simp
+  use k + 1, k + 2 + n, by omega;;
+  simpa [h₁, h, h₃]
+
+@[simp]
+theorem State.simStatesIcoVia_self {s : State} {st} : s.simStatesIcoVia st s = ∅ := by
+  simp [simStatesIcoVia, simStatesRangeAuxVia]
+
+@[simp]
+theorem State.aSimStatesIcoVia_self {s : State} {st} : s.aSimStatesIcoVia st s = ∅ := by
+  simp [aSimStatesIcoVia]
+
+@[simp]
+theorem State.aVisitedIco_self {s : State} : s.aVisitedIco s = ∅ := by
+  simp [aVisitedIco]
+
+theorem State.simStatesIccVia_eq_of_tr {s s₁} {st : Strat} [hs : sys.WF s]
+(h : sys.tr s (st.f s) = some s₁) : s.simStatesIccVia st s₁ = {s, s₁} := by
+  have h' : sys.simulate st.f s 1 = (s₁, 0); simpa
+  ext s'; simp [simStatesIccVia, mem_simStatesRangeAuxVia_iff h']; constructor
+  · rintro ⟨⟨n, h₁⟩, h₂⟩; obtain rfl | rfl : n = 0 ∨ n = 1
+    · have := length_hist_eq_of_tr h; have := length_hist_eq_of_simulate_eq h₁; omega
+    all_goals simp [h] at h₁; grind
+  · rintro (rfl | rfl); all_goals simp [length_hist_eq_of_tr h]
+    use 0; simp; use 1
+
+theorem State.simStatesIcoVia_eq_of_tr {s s₁} {st : Strat}
+(h : sys.tr s (st.f s) = some s₁) : s.simStatesIcoVia st s₁ = {s} := by
+  have h' : sys.simulate st.f s 1 = (s₁, 0); simpa
+  ext s'; simp [simStatesIcoVia, mem_simStatesRangeAuxVia_iff h']; constructor
+  · rintro ⟨⟨n, h₁⟩, h₂⟩; obtain rfl | rfl : n = 0 ∨ n = 1
+    · have := length_hist_eq_of_tr h; have := length_hist_eq_of_simulate_eq h₁; omega
+    all_goals simp [h] at h₁; grind
+  · rintro (rfl | rfl); all_goals simp [length_hist_eq_of_tr h]
+    use 0; simp
+
+theorem State.simStatesIcoVia_eq_simStatesIccVia_prev_of {s s₁ : State} {st : Strat} {n}
+[hs : sys.WF s] (h₁ : sys.simulate st.f s n = (s₁, 0)) (h₂ : n ≠ 0) :
+s.simStatesIcoVia st s₁ = s.simStatesIccVia st s₁.prev := by
+  ext s'
+  cases n
+  · simp at h₂
+  nm n
+  clear h₂
+  have h₁' := h₁
+  simp at h₁
+  choose sx h₁ h₃ using h₁
+  have hsx : sys.WF sx; grind
+  rw [prev_eq_of_tr h₃]
+  simp [simStatesIcoVia_eq_erase_simStatesIccVia, simStatesIccVia]
+  simp [mem_simStatesRangeAuxVia_iff h₁, mem_simStatesRangeAuxVia_iff h₁']
+  constructor
+  · rintro ⟨h₄, ⟨k, h₅⟩, h₆⟩
+    use by use k
+    have := length_hist_eq_of_simulate_eq h₁
+    have := length_hist_eq_of_simulate_eq h₅
+    have := length_hist_eq_of_tr h₃
+    have hk : k ≤ n + 1
+    · omega
+    rw [le_iff_eq_or_lt] at hk
+    rcases hk with rfl | hk
+    · rw [h₁'] at h₅
+      grind
+    omega
+  · rintro ⟨⟨k, h₄⟩, h₅⟩
+    rw [length_hist_eq_of_simulate_eq h₁] at h₅
+    rw [length_hist_eq_of_simulate_eq h₄] at h₅
+    simp at h₅
+    obtain ⟨n, rfl⟩ := Nat.exists_eq_add_of_le h₅
+    clear h₅
+    clear h₁'
+    simp [h₄] at h₁
+    have hs' : sys.WF s'; grind
+    split_ands
+    · rintro rfl
+      apply s'.false_of_simulate_eq_simulate st.f s' s' 0 (n + 1) <;> simp_all
+    · use k
+    · apply length_hist_le_of_reachable
+      apply sys.reachable_of_simulate h₁ |>.trans
+      exact sys.reachable_of_tr h₃
+
+theorem State.aSimStatesIcoVia_eq_aSimStatesIccVia_prev_of {s s₁ : State} {st : Strat} {n}
+[hs : sys.WF s] (h₁ : sys.simulate st.f s n = (s₁, 0)) (h₂ : n ≠ 0) :
+s.aSimStatesIcoVia st s₁ = s.aSimStatesIccVia st s₁.prev := by
+  rw [aSimStatesIcoVia, aSimStatesIccVia, simStatesIcoVia_eq_simStatesIccVia_prev_of h₁ h₂]
+
+theorem State.mem_aVisitedIcoPrev_iff_exi_aSimStatesIcoVia
+{s s₁ : State} {st : Strat} {n p} [hs : AState s] [hs₁ : AState s₁] [hst : st.WF]
+(h₁ : s ≠ s₁) (h₂ : sys.simulate st.f s n = (s₁, 0)) :
+p ∈ s.aVisitedIcoPrev s₁ ↔ ∃ s' ∈ s.aSimStatesIcoVia st s₁, s'.aPos = p := by
+  obtain ⟨n, rfl⟩ := Nat.even_iff_exi.mp # AState.even_of_simulate h₂
+  cases n
+  · simp [h₁] at h₂
+  nm n
+  rw [show (n + 1) * 2 = n * 2 + 2 by omega] at h₂
+  have h₆ := h₂
+  simp at h₂
+  obtain ⟨sd, ⟨sa, h₂, h₃⟩, h₄⟩ := h₂
+  have hsa := AState.of_simulate_mul_two_eq' h₂
+  have hsd := DState.of_tr h₃
+  unfold aVisitedIcoPrev
+  rw [diff_eq_of_simulate h₆, if_neg # by omega, prev_eq_of_tr h₄]
+  have h₅ : sys.simulate st.f s (n * 2 + 1) = (sd, 0); simp_all
+  rw [mem_aVisitedIco_iff_of h₅]
+  simp [mem_aSimStatesIcoVia_iff_of h₆, and_assoc]
+  constructor
+  · rintro (rfl | ⟨k, hk, s', hs', H₁, H₂⟩)
+    · use s; simpa
+    have H₂' := H₂
+    simp at H₂
+    obtain ⟨sx, hsx, H₃⟩ : ∃ sx, DState sx ∧ sys.simulate st.f s (k + 1) = (sx, 0)
+    · simp [H₁, H₂]
+      suffices h : sys.validTr s' p
+      · choose sx h using h
+        use sx, by grind
+      rw [←H₂']
+      apply hst.validTr
+      apply sys.hasTr_of_reachable_and_ne (s₂ := sd)
+      on_goal 2 => grind
+      obtain ⟨c, H₃⟩ := Nat.exists_eq_add_of_lt hk
+      simp [H₃, H₁] at h₂; grind
+    simp [H₁] at H₃
+    obtain ⟨sy, hsy, H₄⟩ : ∃ sy, AState sy ∧ sys.simulate st.f s (k + 2) = (sy, 0)
+    · simp [H₁, H₃]
+      have h : sys.validTr sx (st.d.f sx); simp
+      choose sy h using h
+      use sy, by grind
+    simp [H₁, H₃] at H₄
+    rw [H₂] at H₃
+    use sy, hsy
+    symm; split_ands
+    · rw [DState.aPos_eq_of_tr H₄, AState.aPos_eq_of_tr H₃]
+    use k + 2, by omega
+    simp_all
+  · rintro ⟨s', hs', ⟨k, hk, H₂⟩, H₁⟩
+    obtain ⟨k, rfl⟩ := Nat.even_iff_exi.mp # AState.even_of_simulate H₂
+    cases k
+    · left; symm
+      simp at H₂
+      rwa [H₂]
+    nm k
+    right
+    replace hk : k < n; omega
+    simp [add_mul] at H₂
+    obtain ⟨sy, ⟨sx, H₂, H₃⟩, H₄⟩ := H₂
+    have hsx := AState.of_simulate_mul_two_eq' H₂
+    have hsy := DState.of_tr H₃
+    use k * 2, by omega, sx, hsx, H₂
+    rw [DState.aPos_eq_of_tr H₄, AState.aPos_eq_of_tr H₃] at H₁
+    exact H₁
+
+@[simp]
+theorem State.aVisitedIcoPrev_self {s : State} : s.aVisitedIcoPrev s = ∅ := by
+  simp [aVisitedIcoPrev]
+
+theorem DState.aNbhdsIcoPrev_eq_of_tr {s s₁ s₂ p} [hs : sys.WF s] [hs₁ : DState s₁]
+(h : sys.tr s₁ p = some s₂) (h₁ : sys.Reachable s s₁) : s.aNbhdsIcoPrev s₂ =
+s.aNbhdsIcoPrev s₁ ∪ if s = s₁ then ∅ else s₁.prev.aPos.nbhd (s.pw) := by
+  have h₁' := h₁
+  rw [sys.reachable_iff_exi_trs] at h₁
+  choose ps h₁ using h₁
+  simp [State.aNbhdsIcoPrev, State.aVisitedIcoPrev, State.diff_eq_of_trs_full h₁,
+    State.diff_eq_of_tr h]
+  induction ps using List.reverseRecOn
+  · simp at h₁
+    simp [h₁]
+  nm ps p' ih; clear ih
+  simp at h₁ ⊢
+  choose s' h₁ h₂ using h₁
+  have hs' : sys.WF s'; grind
+  simp [State.prev_eq_of_tr h, State.prev_eq_of_tr h₂]
+  simp [State.aVisitedIco]
+  induction ps using List.reverseRecOn
+  · simp at h₁ ⊢
+    subst h₁
+    split_ifs with h₃; simp
+    ext p₂
+    simp [State.prev_eq_of_tr h₂]
+  nm ps p₂ ih; clear ih
+  simp at h₁ ⊢
+  choose s₀ h₁ h₃ using h₁
+  have hs₀ : sys.WF s₀; grind
+  have H₁ : sys.trs s (ps ++ [p₂, p']) = (s₁, []); simp_all
+  have H₂ : sys.trs s (ps ++ [p₂]) = (s', []); simp_all
+  have H₃ : s ≠ s₁; rintro rfl; have H₃ := State.length_hist_eq_of_trs_eq H₁; simp at H₃
+  have H₄ : s ≠ s'; rintro rfl; have H₃ := State.length_hist_eq_of_trs_eq H₂; simp at H₃
+  simp [H₃, H₄]; ext q
+  simp [State.prev_eq_of_tr h₂, State.prev_eq_of_tr h₃]
+  replace hs' : AState s'; grind
+  replace hs₀ : DState s₀; grind
+  have H₅ : sys.Reachable s s₀; grind
+  obtain ⟨f, hf, n, H₆⟩ := sys.exi_simulate_of_reachable H₅
+  rw [@aVisitedIcc_eq_of_tr s s₀ s' p₂ _ _ h₃ H₅]
+  simp
+  intro H₇
+  use s'.aPos
+  simp [H₇]
+  rw [State.mem_aVisitedIcc_iff_of H₆]
+  cases n
+  · left
+    simp at H₆
+    subst H₆
+    rw [DState.aPos_eq_of_tr h₃]
+  nm n
+  right
+  simp at H₆
+  choose s₃ H₆ H₈ using H₆
+  have hs₃ : AState s₃; grind
+  use n, by omega, s₃, by grind, H₆
+  rw [DState.aPos_eq_of_tr h₃, AState.aPos_eq_of_tr H₈]
