Projects/AP/Moves/Part_002.lean
@@ -1,0 +1,271 @@
+import Projects.AP.Moves.Part_001
+import Projects.Temp
+
+namespace AP
+
+theorem AState.aNbhdsIcoPrev_eq_of_tr {s s₁ s₂ p} [hs : sys.WF s] [hs₁ : AState s₁]
+(h : sys.tr s₁ p = some s₂) (h₁ : sys.Reachable s s₁) :
+s.aNbhdsIcoPrev s₂ = s.aNbhdsIcoPrev s₁ ∪ if s = s₁ then ∅ else s₁.prev.aPos.nbhd (s.pw) := by
+  have h₁' := h₁
+  rw [sys.reachable_iff_exi_trs] at h₁
+  choose ps h₁ using h₁
+  simp [State.aNbhdsIcoPrev, State.aVisitedIcoPrev, State.diff_eq_of_trs_full h₁,
+    State.diff_eq_of_tr h]
+  induction ps using List.reverseRecOn
+  · simp at h₁
+    simp [h₁]
+  nm ps p' ih; clear ih
+  simp at h₁ ⊢
+  choose s' h₁ h₂ using h₁
+  have hs' : sys.WF s'; grind
+  simp [State.prev_eq_of_tr h, State.prev_eq_of_tr h₂]
+  simp [State.aVisitedIco]
+  induction ps using List.reverseRecOn
+  · simp at h₁ ⊢
+    subst h₁
+    split_ifs with h₃; simp
+    ext p₂
+    simp [State.prev_eq_of_tr h₂]
+  nm ps p₂ ih; clear ih
+  simp at h₁ ⊢
+  choose s₀ h₁ h₃ using h₁
+  have hs₀ : sys.WF s₀; grind
+  have H₁ : sys.trs s (ps ++ [p₂, p']) = (s₁, []); simp_all
+  have H₂ : sys.trs s (ps ++ [p₂]) = (s', []); simp_all
+  have H₃ : s ≠ s₁; rintro rfl; have H₃ := State.length_hist_eq_of_trs_eq H₁; simp at H₃
+  have H₄ : s ≠ s'; rintro rfl; have H₃ := State.length_hist_eq_of_trs_eq H₂; simp at H₃
+  simp [H₃, H₄]; ext q
+  simp [State.prev_eq_of_tr h₂, State.prev_eq_of_tr h₃]
+  replace hs' : DState s'; grind
+  replace hs₀ : AState s₀; grind
+  have H₅ : sys.Reachable s s₀; grind
+  obtain ⟨f, hf, n, H₆⟩ := sys.exi_simulate_of_reachable H₅
+  rw [@aVisitedIcc_eq_of_tr s s₀ s' p₂ _ _ h₃ H₅]
+  nth_rw 1 [or_comm]
+  simp
+  congr!
+  rw [AState.aPos_eq_of_tr h₃]
+
+theorem State.aNbhdsIcoPrev_eq_of_tr {s s₁ s₂ p} [hs : sys.WF s]
+(h : sys.tr s₁ p = some s₂) (h₁ : sys.Reachable s s₁) :
+s.aNbhdsIcoPrev s₂ = s.aNbhdsIcoPrev s₁ ∪ if s = s₁ then ∅ else s₁.prev.aPos.nbhd (s.pw) := by
+  have hs₁ : sys.WF s₁; grind
+  replace hs₁ := s₁.aState_or_dState
+  rcases hs₁ with hs₁ | hs₁
+  · exact AState.aNbhdsIcoPrev_eq_of_tr h h₁
+  · exact DState.aNbhdsIcoPrev_eq_of_tr h h₁
+
+@[simp]
+theorem State.aNbhdsIcoPrev_self {s : State} : s.aNbhdsIcoPrev s = ∅ := by
+  simp [aNbhdsIcoPrev]
+
+@[simp]
+instance init_reachable {s} [hs : sys.WF s] : sys.Reachable s.init s := by
+  rw [State.wf_iff'] at hs; rw [State.init]; grind
+
+theorem State.wf_iff {s} : sys.WF s ↔ ∃ ps, sys.trs s.init ps = (s, []) := by
+  rw [sys.wf_def]; constructor
+  · rintro ⟨s₀, h₁, h₂⟩
+    have h₃ := h₁
+    have h₄ := h₂
+    rw [sys.reachable_iff_exi_trs] at h₂
+    choose ps h₂ using h₂
+    use ps
+    rw [init]
+    rw [initial_iff] at h₁
+    rwa [pw_eq_of_reachable h₄, aPos₀_eq_of_reachable h₄, h₁]
+  · rintro ⟨ps, h⟩
+    have hs : sys.WF s; grind
+    use s.init
+    simp; simp [init]
+
+theorem init_eq_of_tr {s s₁ p} [hs : sys.WF s]
+(h : sys.tr s p = some s₁) : s₁.init = s.init := by
+  simp [State.init, pw_eq_of_tr h, State.aPos₀_eq_of_tr h]
+
+theorem init_eq_of_trs {s s₁ ps ps'} [hs : sys.WF s]
+(h : sys.trs s ps = (s₁, ps')) : s₁.init = s.init := by
+  replace h := sys.exi_trs_full_of_trs h
+  choose ps₁ h₁ h₂ using h
+  clear! ps
+  rename' ps₁ => ps
+  induction ps using List.reverseRecOn generalizing s₁
+  · simp at h₂; rw [h₂]
+  nm ps₁ p ih
+  simp at h₂
+  choose s' h₂ h₃ using h₂
+  specialize ih h₂
+  have hs' : sys.WF s'; grind
+  grind [init_eq_of_tr h₃]
+
+theorem init_eq_of_reachable {s s₁} [hs : sys.WF s]
+(h : sys.Reachable s s₁) : s₁.init = s.init := by
+  rw [sys.reachable_iff_exi_trs] at h; choose ps h using h; exact init_eq_of_trs h
+
+@[simp]
+theorem State.odd_length_hist {s} [hs : sys.WF s] : Odd s.hist.length ↔ s.aTurn = false := by
+  rw [wf_iff] at hs
+  choose ps h using hs
+  induction ps using List.reverseRecOn generalizing s
+  · simp at h; rw [←h]; simp
+  nm ps p ih
+  simp at h
+  choose s₁ h₁ h₂ using h
+  have hs₁ : sys.WF s₁; grind
+  rw [init_eq_of_tr h₂] at h₁
+  specialize ih h₁
+  rw [length_hist_eq_of_tr h₂, aTurn_eq_of_tr h₂]
+  contrapose!; simpa
+
+@[simp]
+theorem State.even_length_hist {s} [hs : sys.WF s] : Even s.hist.length ↔ s.aTurn = true := by
+  contrapose!; simp
+
+@[simp]
+theorem State.odd_length_hist_sub_one {s} [hs : sys.WF s] :
+Odd (s.hist.length - 1) ↔ s.aTurn = true := by
+  rw [←Nat.odd_add_two, length_hist_sub_one_add]; simp
+
+@[simp]
+theorem State.even_length_hist_sub_one {s} [hs : sys.WF s] :
+Even (s.hist.length - 1) ↔ s.aTurn = false := by
+  rw [←Nat.even_add_two, length_hist_sub_one_add]; simp
+
+@[simp] theorem taken_init {s : State} : s.init.taken = ∅ := rfl
+@[simp] theorem aPos_init {s : State} : s.init.aPos = s.aPos₀ := rfl
+@[simp] theorem hist_init {s : State} : s.init.hist = [s.aPos₀] := rfl
+@[simp] theorem init_init {s : State} : s.init.init = s.init := rfl
+
+@[simp] theorem Strat.a_ofFn {f} : (ofFn f).a = .mk f := rfl
+@[simp] theorem Strat.d_ofFn {f} : (ofFn f).d = .mk f := rfl
+
+@[simp, instance]
+theorem Strat.wf_ofFn {f} : ofFn f |>.WF := by
+  simp [wf_iff]
+
+@[simp]
+theorem Strat.f_ofFn {f} : (ofFn f).f = mkStratFn f := by
+  ext s :1; simp [ofFn, Strat.f]
+
+theorem State.eq_of_reachable_and_hist_eq {s s₁ s₂} (h₁ : sys.Reachable s s₁)
+(h₂ : sys.Reachable s s₂) (h₃ : s₁.hist = s₂.hist) : s₁ = s₂ := by
+  rw [System.reachable_iff_exi_trs] at h₁ h₂
+  choose ps₁ h₁ using h₁
+  choose ps₂ h₂ using h₂
+  have h₄ := hist_eq_of_trs h₁
+  have h₅ := hist_eq_of_trs h₂
+  simp at h₄ h₅
+  simp [h₃] at h₄
+  simp [h₄] at h₅
+  subst h₅
+  simp [h₁] at h₂
+  exact h₂
+
+theorem State.eq_of_reachable_and_length_hist_eq {s s₁ s₂ s₃}
+(h₁ : sys.Reachable s s₁) (h₂ : sys.Reachable s s₂) (h₃ : sys.Reachable s₁ s₃)
+(h₄ : sys.Reachable s₂ s₃) (h₅ : s₁.hist.length = s₂.hist.length) : s₁ = s₂ := by
+  apply eq_of_reachable_and_hist_eq h₁ h₂
+  apply List.eq_of_suffix_and_length_eq (zs := s₃.hist) _ _ h₅
+  · exact hist_suffix_of_reachable h₃
+  · exact hist_suffix_of_reachable h₄
+
+theorem point_eq_of_tr_eq_tr {s s' p₁ p₂} (h₁ : sys.tr s p₁ = some s')
+(h₂ : sys.tr s p₂ = some s') : p₁ = p₂ := by
+  have h₃ := hist_eq_of_tr h₁
+  have h₄ := hist_eq_of_tr h₂
+  simp [h₃] at h₄
+  exact h₄
+
+-- #check 0 #exit
+
+-- theorem State.simulate_diffStrat {s s₁} [hs : sys.WF s] (h : sys.Reachable s s₁) :
+-- sys.simulate (s.diffStrat s₁).f s (s.diff s₁) = (s₁, 0) := by
+--   obtain ⟨f, hf, n, h₁⟩ := sys.reachable_iff_exi_simulate.mp h
+--   obtain ⟨ps, h₂⟩ := sys.reachable_iff_exi_trs.mp h
+--   
+--   have hn : ps.length = n
+--   ·
+--     have h₃ := length_hist_eq_of_simulate_eq h₁
+--     have h₄ := length_hist_eq_of_trs_eq h₂
+--     grind
+--   
+--   generalize hg : (s.diffStrat s₁).f = g
+--   
+--   replace hg : ∀ ⦃s'⦄, (∃ k < n, sys.simulate f s k = (s', 0)) →
+--     g s' = (s.diffTrs s₁)[s.diff s']!
+--   ·
+--     rintro s' ⟨k, hk, h₃⟩
+--     subst hg
+--     simp [diffStrat, diffTrs_eq_of_trs_full h₂, diff_eq_of_simulate_full h₃]
+--     obtain ⟨ps₁, ps₂, p, H₁, rfl⟩ : ∃ (ps₁ ps₂ : List PointZ) (p : PointZ),
+--       ps₁.length = k ∧ ps₁ ++ p :: ps₂ = ps
+--     ·
+--       use ps.take k, ps.drop (k + 1), ps[k]!
+--       simp
+--       use by omega
+--       rw [List.ext_getElem_iff]
+--       simp
+--       grind
+--     subst H₁
+--     simp at hn ⊢
+--     subst hn
+--     rw [add_comm _ 1] at h₁
+--     simp at h₁
+--     choose sx h₁ sy h₄ h₅ using h₁
+--     simp [h₃] at h₁
+--     subst h₁
+--     -- simp [sys.validTr_of_eq_some h₄]
+--     simp at h₂
+--     choose sx' h₂ sy' h₆ h₇ using h₂
+--     obtain rfl : sx' = s'
+--     ·
+--       apply eq_of_reachable_and_length_hist_eq (s := s) (s₃ := s₁)
+--       iterate 4 grind
+--       rw [length_hist_eq_of_simulate_eq h₃, length_hist_eq_of_trs_eq h₂]
+--       rfl
+--     rename' sx' => sx
+--     obtain rfl : sy = sy'
+--     ·
+--       apply eq_of_reachable_and_length_hist_eq (s := sx) (s₃ := s₁)
+--       iterate 4 grind
+--       rw [length_hist_eq_of_tr h₆, length_hist_eq_of_tr h₄]
+--     obtain rfl := point_eq_of_tr_eq_tr h₄ h₆
+--     simp [sys.validTr_of_eq_some h₆]
+--   
+--   apply And.right (a := n = 0 ∨ ∃ k < n, sys.simulate f s k = (s, 0))
+--   rw [diff_eq_of_simulate_full h₁]
+--   
+--   induction n generalizing s ps; simp_all
+--   nm n ih
+--   rw [System.simulate_succ_full'] at h₁ ⊢
+--   choose sx h₁ h₃ using h₁
+--   simp
+--   use sx
+--   cases ps
+--   ·
+--     clear ih
+--     exfalso
+--     simp at h₂
+--     subst h₂
+--     have h₄ := sys.reachable_of_tr h₁
+--     have h₅ := sys.reachable_of_simulate h₃
+--     have h₆ := sys.eq_of_tree_and_reachable h₄ h₅
+--     simp [h₆] at h₁
+--   nm p ps
+--   simp at h₂ hn
+--   choose sx' h₂ h₄ using h₂
+--   obtain rfl : sx = sx'
+--   ·
+--     apply eq_of_reachable_and_length_hist_eq (s := s) (s₃ := s₁)
+--     iterate 4 grind
+--     rw [length_hist_eq_of_tr h₁, length_hist_eq_of_tr h₂]
+--   obtain rfl := point_eq_of_tr_eq_tr h₁ h₂
+--   clear h₂
+--   have hsx : sys.WF sx; grind
+--   
+--   specialize @ih sx _ (by grind) h₃ ps h₄ hn _
+--   ·
+--     clear ih
+--     rintro s' ⟨k, hk, H⟩
+--     sorry
+--   sorry
