Projects/AP/Proximity.lean
@@ -1,0 +1,43 @@
+import Projects.AP.Moves
+
+namespace AP
+
+open Classical in noncomputable
+def State.aProx (s s₁ : State) : Set' PointZ :=
+  Set'.ofSet # setOf λ p => sys.WF s ∧ sys.Reachable s s₁ ∧
+  (∃ ps s₂, ps <+: s₁.diffTrs s ∧ sys.trs s ps = (s₂, []) ∧ s₂.aPos = p) ∧
+  ∃ ps p₁ s₂, AState s₂ ∧ ps ++ [p₁] <+: s₁.diffTrs s ∧ sys.trs s ps = (s₂, []) ∧
+    sys.validTr s₂ p ∧ p ≠ p₁
+
+def State.aProx' (s s₁ : State) : Set' PointZ :=
+  s.aNbhdsIcoPrev s₁
+
+-----
+
+-- theorem State.aux₁ {s s₁ : State} [hs : sys.WF s] {p} :
+-- p ∈ s.aNbhdsIcoPrev s₁ ↔ sys.WF s ∧ sys.Reachable s s₁ ∧
+-- (∃ ps, ps <+: s₁.diffTrs s ∧ ∃ x, sys.trs s ps = (x, []) ∧ x.aPos = p) ∧
+-- ∃ ps p₁ s₂, AState s₂ ∧ ps ++ [p₁] <+: s₁.diffTrs s ∧ sys.trs s ps = (s₂, []) ∧
+-- sys.validTr s₂ p ∧ ¬p = p₁ := by
+--   simp [aNbhdsIcoPrev, hs]
+--   constructor
+--   ·
+--     rintro ⟨p₁, h₁, h₂⟩
+--     rw [mem_aVisitedIcoPrev_iff_exi_aSimStatesIco] at h₁
+-- 
+-- -- #check 0 #exit
+-- 
+-- theorem State.aPox_eq_aPox' {s s₁ : State} [hs : sys.WF s] : s.aProx s₁ = s.aProx' s₁ := by
+--   unfold aProx aProx'
+--   ext p
+--   rw [Set'.mem_ofSet]
+--   rotate_left
+--   ·
+--     rw [Set.finite_iff_exi_finset]
+--     use s.aNbhdsIcoPrev s₁ |>.toFinset
+--     clear p
+--     ext p
+--     simp
+--     exact aux₁
+--   simp
+--   exact aux₁.symm
